Reverted Registers, Tensor_Product, With_Type to afp-devel

thys/Registers/Axioms_Quantum.thy
@@ -3,7 +3,7 @@ section \<open>Quantum instantiation of registers\<close>
 (* AXIOM INSTANTIATION (use instantiate_laws.py to generate Laws_Quantum.thy)
 
     # Type classes
-    domain \<rightarrow> type
+    domain \<rightarrow> finite
 
     # Types
     some_domain \<rightarrow> unit
@@ -11,13 +11,18 @@ section \<open>Quantum instantiation of registers\<close>
     # Constants
     comp_update \<rightarrow> cblinfun_compose
     id_update \<rightarrow> id_cblinfun
+    preregister \<rightarrow> clinear
     tensor_update \<rightarrow> tensor_op
     
     # Lemmas
     id_update_left \<rightarrow> cblinfun_compose_id_left
     id_update_right \<rightarrow> cblinfun_compose_id_right
     comp_update_assoc \<rightarrow> cblinfun_compose_assoc
+    id_preregister \<rightarrow> complex_vector.linear_id
+    comp_preregister \<rightarrow> clinear_compose
     tensor_update_mult \<rightarrow> comp_tensor_op
+    # preregister_tensor_left \<rightarrow> clinear_tensor_right
+    # preregister_tensor_right \<rightarrow> clinear_tensor_left
 
     # Chapter name
     Generic laws about registers \<rightarrow> Generic laws about registers, instantiated quantumly
@@ -27,9 +32,7 @@ section \<open>Quantum instantiation of registers\<close>
 theory Axioms_Quantum
   imports Jordan_Normal_Form.Matrix_Impl "HOL-Library.Rewrite"
           Complex_Bounded_Operators.Complex_L2
-          (* Finite_Tensor_Product *)
-          Tensor_Product.Hilbert_Space_Tensor_Product
-          Tensor_Product.Weak_Star_Topology
+          Finite_Tensor_Product
 begin
 
 
@@ -38,32 +41,14 @@ no_notation m_inv ("inv\<index> _" [81] 80)
 
 type_synonym 'a update = \<open>('a ell2, 'a ell2) cblinfun\<close>
 
-definition preregister :: \<open>('a update \<Rightarrow> 'b update) \<Rightarrow> bool\<close> where
-  \<open>preregister F \<longleftrightarrow> bounded_clinear F \<and> continuous_map weak_star_topology weak_star_topology F\<close>
+lemma preregister_mult_right: \<open>clinear (\<lambda>a. a o\<^sub>C\<^sub>L z)\<close>
+  by (simp add: bounded_cbilinear.add_left bounded_cbilinear_cblinfun_compose clinearI)
+lemma preregister_mult_left: \<open>clinear (\<lambda>a. z o\<^sub>C\<^sub>L a)\<close>
+  by (meson cbilinear_cblinfun_compose cbilinear_def)
 
-lemma preregister_mult_right: \<open>preregister (\<lambda>a. a o\<^sub>C\<^sub>L z)\<close>
-  apply (auto simp add: bounded_cbilinear.bounded_clinear_left bounded_cbilinear_cblinfun_compose
-      preregister_def)
-  sorry
-lemma preregister_mult_left: \<open>preregister (\<lambda>a. z o\<^sub>C\<^sub>L a)\<close>
-  apply (auto simp add: bounded_cbilinear.bounded_clinear_right bounded_cbilinear_cblinfun_compose
-      preregister_def)
-  sorry
-
-lemma comp_preregister: "preregister F \<Longrightarrow> preregister G \<Longrightarrow> preregister (G \<circ> F)"
-  by (auto simp add: preregister_def continuous_map_compose comp_bounded_clinear)
-
-lemma id_preregister: \<open>preregister id\<close>
-  unfolding preregister_def by auto
-
-lemma tensor_extensionality:
-  \<open>preregister F \<Longrightarrow> preregister G \<Longrightarrow> (\<And>a b. F (tensor_op a b) = G (tensor_op a b)) \<Longrightarrow> F = G\<close>
-  sorry
-
-definition register :: \<open>('a update \<Rightarrow> 'b update) \<Rightarrow> bool\<close> where
+definition register :: \<open>('a::finite update \<Rightarrow> 'b::finite update) \<Rightarrow> bool\<close> where
   "register F \<longleftrightarrow> 
-     bounded_clinear F
-   \<and> continuous_map weak_star_topology weak_star_topology F
+     clinear F
    \<and> F id_cblinfun = id_cblinfun 
    \<and> (\<forall>a b. F(a o\<^sub>C\<^sub>L b) = F a o\<^sub>C\<^sub>L F b)
    \<and> (\<forall>a. F (a*) = (F a)*)"
@@ -74,31 +59,29 @@ lemma register_of_id: \<open>register F \<Longrightarrow> F id_cblinfun = id_cbl
 lemma register_id: \<open>register id\<close>
   by (simp add: register_def complex_vector.module_hom_id)
 
-lemma register_preregister: "register F \<Longrightarrow> preregister F"
-  unfolding register_def preregister_def by auto
+lemma register_preregister: "register F \<Longrightarrow> clinear F"
+  unfolding register_def by simp
 
 lemma register_comp: "register F \<Longrightarrow> register G \<Longrightarrow> register (G \<circ> F)"
-  using bounded_clinear_compose continuous_map_compose apply (auto simp: o_def register_def)
-  by blast
+  unfolding register_def
+  apply auto
+  using clinear_compose by blast
 
 lemma register_mult: "register F \<Longrightarrow> cblinfun_compose (F a) (F b) = F (cblinfun_compose a b)"
   unfolding register_def
   by auto
 
 lemma register_tensor_left: \<open>register (\<lambda>a. tensor_op a id_cblinfun)\<close>
-  apply (auto simp add: comp_tensor_op register_def tensor_op_cbilinear tensor_op_adjoint)
-  apply (metis eq_onp_def right_amplification.rsp)
-  sorry
+  by (simp add: comp_tensor_op register_def tensor_op_cbilinear tensor_op_adjoint)
 
 lemma register_tensor_right: \<open>register (\<lambda>a. tensor_op id_cblinfun a)\<close>
-  apply (auto simp add: comp_tensor_op register_def tensor_op_cbilinear tensor_op_adjoint)
-  sorry
+  by (simp add: comp_tensor_op register_def tensor_op_cbilinear tensor_op_adjoint)
 
 definition register_pair ::
-  \<open>('a update \<Rightarrow> 'c update) \<Rightarrow> ('b update \<Rightarrow> 'c update)
+  \<open>('a::finite update \<Rightarrow> 'c::finite update) \<Rightarrow> ('b::finite update \<Rightarrow> 'c update)
          \<Rightarrow> (('a\<times>'b) update \<Rightarrow> 'c update)\<close> where
   \<open>register_pair F G = (if register F \<and> register G \<and> (\<forall>a b. F a o\<^sub>C\<^sub>L G b = G b o\<^sub>C\<^sub>L F a) then 
-                        SOME R. (\<forall>a b. register R \<and> R (a\<otimes>\<^sub>ob) = F a o\<^sub>C\<^sub>L G b) else (\<lambda>_. 0))\<close>
+                        tensor_lift (\<lambda>a b. F a o\<^sub>C\<^sub>L G b) else (\<lambda>_. 0))\<close>
 
 lemma cbilinear_F_comp_G[simp]: \<open>clinear F \<Longrightarrow> clinear G \<Longrightarrow> cbilinear (\<lambda>a b. F a o\<^sub>C\<^sub>L G b)\<close>
   unfolding cbilinear_def
@@ -108,18 +91,16 @@ lemma register_pair_apply:
   assumes [simp]: \<open>register F\<close> \<open>register G\<close>
   assumes \<open>\<And>a b. F a o\<^sub>C\<^sub>L G b = G b o\<^sub>C\<^sub>L F a\<close>
   shows \<open>(register_pair F G) (tensor_op a b) = F a o\<^sub>C\<^sub>L G b\<close>
-(*   unfolding register_pair_def
+  unfolding register_pair_def
   apply (simp flip: assms(3))
-  by (metis assms(1) assms(2) cbilinear_F_comp_G register_preregister tensor_lift_correct)x *)
-  sorry
+  by (metis assms(1) assms(2) cbilinear_F_comp_G register_preregister tensor_lift_correct)
 
 lemma register_pair_is_register:
-  fixes F :: \<open>'a update \<Rightarrow> 'c update\<close> and G
+  fixes F :: \<open>'a::finite update \<Rightarrow> 'c::finite update\<close> and G
   assumes [simp]: \<open>register F\<close> and [simp]: \<open>register G\<close>
   assumes \<open>\<And>a b. F a o\<^sub>C\<^sub>L G b = G b o\<^sub>C\<^sub>L F a\<close>
   shows \<open>register (register_pair F G)\<close> 
-  sorry
-(* proof (unfold register_def, intro conjI allI)
+proof (unfold register_def, intro conjI allI)
   have [simp]: \<open>clinear F\<close> \<open>clinear G\<close>
     using assms register_def by blast+
   have [simp]: \<open>F id_cblinfun = id_cblinfun\<close> \<open>G id_cblinfun = id_cblinfun\<close>
@@ -149,14 +130,14 @@ lemma register_pair_is_register:
     by (simp add: register_mult)
   have [simp]: \<open>G (x o\<^sub>C\<^sub>L y) = G x o\<^sub>C\<^sub>L G y\<close> for x y
     by (simp add: register_mult)
-  have [simp]: \<open>clinear (\<lambda>a. (register_pair F G (a* ))* )\<close>
+  have [simp]: \<open>clinear (\<lambda>a. (register_pair F G (a*))*)\<close>
     apply (rule antilinear_o_antilinear[unfolded o_def, where f=\<open>adj\<close>])
      apply simp
     apply (rule antilinear_o_clinear[unfolded o_def, where g=\<open>adj\<close>])
     by (simp_all)
-  have [simp]: \<open>F (a* ) = (F a)*\<close> for a
+  have [simp]: \<open>F (a*) = (F a)*\<close> for a
     using assms(1) register_def by blast
-  have [simp]: \<open>G (b* ) = (G b)*\<close> for b
+  have [simp]: \<open>G (b*) = (G b)*\<close> for b
     using assms(2) register_def by blast
 
   fix a b
@@ -166,11 +147,11 @@ lemma register_pair_is_register:
     apply (simp_all add: comp_tensor_op register_pair_apply assms(3))
     using assms(3)
     by (metis cblinfun_compose_assoc)
-  have \<open>(register_pair F G (a* ))* = register_pair F G a\<close>
+  have \<open>(register_pair F G (a*))* = register_pair F G a\<close>
     apply (rule tensor_extensionality[THEN fun_cong, where x=a])
     by (simp_all add: tensor_op_adjoint register_pair_apply assms(3))
-  then show \<open>register_pair F G (a* ) = register_pair F G a*\<close>
+  then show \<open>register_pair F G (a*) = register_pair F G a*\<close>
     by (metis double_adj)
-qed *)
+qed
 
 end
