thys/Registers/Axioms_Complement_Quantum.thy
@@ -1,876 +1,285 @@
 section \<open>Quantum instantiation of complements\<close>
 
 theory Axioms_Complement_Quantum
-  imports Laws_Quantum With_Type.With_Type_Inst_Complex_Bounded_Operators Quantum_Extra Tensor_Product.Weak_Star_Topology
-    Tensor_Product.Partial_Trace
+  imports Laws_Quantum Finite_Tensor_Product Quantum_Extra
 begin
 
 no_notation m_inv ("inv\<index> _" [81] 80)
 no_notation Lattice.join (infixl "\<squnion>\<index>" 65)
-no_notation elt_set_eq (infix "=o" 50)
-no_notation eq_closure_of ("closure'_of\<index>")
 
-(* lemma finite_subsets_at_top_parametric[transfer_rule]:
-  includes lifting_syntax
-  assumes [transfer_rule]: \<open>bi_unique R\<close>
-  shows \<open>(rel_set R ===> rel_filter (rel_set R)) finite_subsets_at_top finite_subsets_at_top\<close>
+typedef ('a::finite,'b::finite) complement_domain = \<open>{..< if CARD('b) div CARD('a) \<noteq> 0 then CARD('b) div CARD('a) else 1}\<close>
+  by auto
+
+instance complement_domain :: (finite, finite) finite
+proof intro_classes
+  have \<open>inj Rep_complement_domain\<close>
+    by (simp add: Rep_complement_domain_inject inj_on_def)
+  moreover have \<open>finite (range Rep_complement_domain)\<close>
+    by (metis finite_lessThan type_definition.Rep_range type_definition_complement_domain)
+  ultimately show \<open>finite (UNIV :: ('a,'b) complement_domain set)\<close>
+    using finite_image_iff by blast
+qed
+
+lemma CARD_complement_domain: 
+  assumes \<open>CARD('b::finite) = n * CARD('a::finite)\<close>
+  shows \<open>CARD(('a,'b) complement_domain) = n\<close>
 proof -
-  have \<open>\<exists>Z. (\<forall>\<^sub>F (S', T') in Z. rel_set R S' T')
-          \<and> map_filter_on {(x, y). rel_set R x y} fst Z = finite_subsets_at_top S
-          \<and> map_filter_on {(x, y). rel_set R x y} snd Z = finite_subsets_at_top T\<close>
-    if \<open>rel_set R S T\<close> for S T
-  proof -
-    from that \<open>bi_unique R\<close>
-    obtain s2t where T_s2t_S: "T = s2t ` S" and "inj_on s2t S" and R_s2t: "\<forall>x\<in>S. R x (s2t x)"
-      using bi_unique_rel_set_lemma by blast
-    define Z where \<open>Z = filtermap (\<lambda>S. (S, s2t ` S)) (finite_subsets_at_top S)\<close>
-    have R_S2T: \<open>rel_set R S' (s2t ` S')\<close> if \<open>S' \<subseteq> S\<close> for S'
-      by (smt (verit, ccfv_threshold) R_s2t \<open>inj_on s2t S\<close> f_inv_into_f in_mono inj_on_image_mem_iff inv_into_into rel_setI that)
-    then have ev_R: \<open>\<forall>\<^sub>F (S', T') in Z. rel_set R S' T'\<close>
-      by (auto simp: Z_def eventually_filtermap intro!: eventually_finite_subsets_at_top_weakI)
-    have 1: \<open>map_filter_on {(x, y). rel_set R x y} fst Z = finite_subsets_at_top S\<close>
-      apply (simp add: filter_eq_iff eventually_map_filter_on ev_R)
-      by (simp add: Z_def eventually_filtermap R_S2T eventually_finite_subsets_at_top)
-    note More_List.no_leading_Cons[rule del]
-    have P_s2t: \<open>S' \<subseteq> S \<Longrightarrow> finite T' \<Longrightarrow> s2t ` S' \<subseteq> T' \<Longrightarrow> T' \<subseteq> T \<Longrightarrow> P T'\<close> 
-      if P: \<open>\<forall>S''. finite S'' \<and> S' \<subseteq> S'' \<and> S'' \<subseteq> S \<longrightarrow> P (s2t ` S'')\<close>
-      for S' P T'
-      using P[rule_format, of \<open>inv_into S s2t ` T'\<close>]
-      by (metis T_s2t_S \<open>inj_on s2t S\<close> equalityE finite_imageI image_inv_into_cancel image_mono inv_into_image_cancel)
-
-    have 2: \<open>map_filter_on {(x, y). rel_set R x y} snd Z = finite_subsets_at_top T\<close>
-      apply (simp add: filter_eq_iff eventually_map_filter_on ev_R)
-      apply (simp add: Z_def eventually_filtermap R_S2T eventually_finite_subsets_at_top)
-      apply (intro allI Ex_iffI[where f=\<open>image s2t\<close> and g=\<open>image (inv_into S s2t)\<close>])
-       apply (safe intro!: intro: P_s2t)
-        (* Sledgehammer proofs below *)
-           apply blast
-          using T_s2t_S apply blast
-         apply (metis P_s2t)
-        apply blast
-       apply (metis T_s2t_S in_mono inv_into_into)
-      by (metis T_s2t_S finite_imageI image_inv_into_cancel image_mono)
-
-    from ev_R 1 2
-    show ?thesis
-      by auto
-  qed
-  then show ?thesis
-    by (simp add: rel_filter.simps rel_funI)
-qed *)
-
-(* TODO: do we even need this, given sum_parametric'? *)
-(* lemma sum_weak_star_transfer[transfer_rule]:
-  includes lifting_syntax
-  fixes R :: \<open>'a \<Rightarrow> 'b \<Rightarrow> bool\<close>
-  assumes [transfer_rule]: \<open>bi_unique R\<close>
-  shows \<open>((R ===> cr_cblinfun_weak_star) ===> rel_set R ===> cr_cblinfun_weak_star) sum sum\<close>
-  apply (rule sum_parametric')
-    apply transfer_step
-    apply transfer_prover
-  by transfer_prover *)
-(* proof (intro rel_funI, rename_tac f g A B)
-  fix f :: \<open>'a \<Rightarrow> 'c \<Rightarrow>\<^sub>C\<^sub>L 'd\<close> and g A B
-  assume Rfg[transfer_rule]: \<open>(R ===> cr_cblinfun_weak_star) f g\<close>
-  assume [transfer_rule]: \<open>rel_set R A B\<close>
-  with \<open>bi_unique R\<close>
-  obtain m where BFA: "B = m ` A" and inj: "inj_on m A" and Rf: "\<forall>x\<in>A. R x (m x)"
-    using bi_unique_rel_set_lemma by blast
-  show \<open>cr_cblinfun_weak_star (sum f A) (sum g B)\<close>
-    apply (subst BFA) using inj Rf
-  proof (induction A rule:infinite_finite_induct)
-    case (infinite A)
-    then show ?case
-      by (auto simp: zero_cblinfun_weak_star.transfer)
-  next
-    case empty
-    show ?case
-      by (auto simp: zero_cblinfun_weak_star.transfer)
-  next
-    case (insert x F)
-    have \<open>cr_cblinfun_weak_star (f x + a) (g y + b)\<close>
-      if [transfer_rule]: \<open>cr_cblinfun_weak_star a b\<close> and [transfer_rule]: \<open>R x y\<close> for a b y
-      by transfer_prover
-    with insert show ?case
-      by simp
-  qed
-qed *)
-
-(* TODO: can we use a generic rule similar to sum_parametric' instead? *)
-lemma has_sum_weak_star_transfer[transfer_rule]:
-  includes lifting_syntax
-  fixes R :: \<open>'a \<Rightarrow> 'b \<Rightarrow> bool\<close>
-  assumes [transfer_rule]: \<open>bi_unique R\<close>
-  shows \<open>((R ===> cr_cblinfun_weak_star) ===> (rel_set R) ===> cr_cblinfun_weak_star ===> (\<longleftrightarrow>)) (has_sum_in weak_star_topology) has_sum\<close>
-  unfolding has_sum_euclidean_iff[symmetric]
-  by transfer_prover
-
-lemma summable_on_weak_star_transfer[transfer_rule]:
-  includes lifting_syntax
-  fixes R :: \<open>'a \<Rightarrow> 'b \<Rightarrow> bool\<close>
-  assumes [transfer_rule]: \<open>bi_unique R\<close>
-  shows \<open>((R ===> cr_cblinfun_weak_star) ===> (rel_set R) ===> (\<longleftrightarrow>)) (summable_on_in weak_star_topology) Infinite_Sum.summable_on\<close>
-(* TODO: can we use a generic rule similar to sum_parametric' instead? *)
-  unfolding summable_on_def summable_on_in_def
-  by transfer_prover
-
-
-lemma infsum_weak_star_transfer[transfer_rule]:
-  includes lifting_syntax
-  fixes R :: \<open>'a \<Rightarrow> 'b \<Rightarrow> bool\<close>
-  assumes [transfer_rule]: \<open>bi_unique R\<close>
-  shows \<open>((R ===> cr_cblinfun_weak_star) ===> (rel_set R) ===> cr_cblinfun_weak_star) (infsum_in weak_star_topology) infsum\<close>
-(* TODO: can we use a generic rule similar to sum_parametric' instead? *)
-proof (intro rel_funI, rename_tac f g A B)
-  fix f :: \<open>'a \<Rightarrow> 'c \<Rightarrow>\<^sub>C\<^sub>L 'd\<close> and g A B
-  assume [transfer_rule]: \<open>(R ===> cr_cblinfun_weak_star) f g\<close>
-  assume [transfer_rule]: \<open>rel_set R A B\<close>
-  show \<open>cr_cblinfun_weak_star (infsum_in Weak_Star_Topology.weak_star_topology f A) (infsum g B)\<close>
-  proof (cases \<open>g summable_on B\<close>)
-    case True
-    then have True': \<open>summable_on_in weak_star_topology f A\<close>
-      apply transfer by simp
-    define a b where \<open>a = infsum_in weak_star_topology f A\<close> and \<open>b = infsum g B\<close>
-    from True' have 1: \<open>has_sum_in weak_star_topology f A a\<close>
-      by (simp add: a_def has_sum_in_infsum_in)
-    from True have \<open>has_sum g B b\<close>
-      using b_def summable_iff_has_sum_infsum by blast
-    then have 2: \<open>b' = b\<close> if \<open>has_sum g B b'\<close> for b'
-      using infsumI that by blast
-    from 1 2 show \<open>cr_cblinfun_weak_star a b\<close>
-      unfolding cr_cblinfun_weak_star_def
-      apply transfer
-      by simp
-  next
-    case False
-    then have False': \<open>\<not> summable_on_in weak_star_topology f A\<close>
-      apply transfer by simp
-    then show ?thesis
-      by (simp add: False infsum_not_exists not_summable_infsum_in_0 zero_cblinfun_weak_star.transfer)
-  qed
+  from assms have \<open>n > 0\<close>
+    by (metis zero_less_card_finite zero_less_mult_pos2)
+  have *: \<open>inj Rep_complement_domain\<close>
+    by (simp add: Rep_complement_domain_inject inj_on_def)
+  moreover have \<open>card (range (Rep_complement_domain :: ('a,'b) complement_domain \<Rightarrow> _)) = n\<close>
+    apply (subst type_definition.Rep_range[OF type_definition_complement_domain])
+    using assms \<open>n > 0\<close> by simp
+  ultimately show ?thesis
+    by (metis card_image)
 qed
 
-definition \<open>register_decomposition_basis \<Phi> = (SOME B. is_ortho_set B \<and> (\<forall>b\<in>B. norm b = 1) \<and> ccspan B = \<Phi> (selfbutterket undefined) *\<^sub>S \<top>)\<close> 
-  for \<Phi> :: \<open>'a update \<Rightarrow> 'b update\<close>
-
-lemma bounded_clinear_cblinfun_compose_left: \<open>bounded_clinear (\<lambda>x. x o\<^sub>C\<^sub>L y)\<close>
-  by (simp add: bounded_cbilinear.bounded_clinear_left bounded_cbilinear_cblinfun_compose)
-lemma bounded_clinear_cblinfun_compose_right: \<open>bounded_clinear (\<lambda>y. x o\<^sub>C\<^sub>L y)\<close>
-  by (simp add: bounded_cbilinear.bounded_clinear_right bounded_cbilinear_cblinfun_compose)
-lemma clinear_cblinfun_compose_left: \<open>clinear (\<lambda>x. x o\<^sub>C\<^sub>L y)\<close>
-  by (simp add: bounded_cbilinear.bounded_clinear_left bounded_cbilinear_cblinfun_compose bounded_clinear.clinear)
-lemma clinear_cblinfun_compose_right: \<open>clinear (\<lambda>y. x o\<^sub>C\<^sub>L y)\<close>
-  by (simp add: bounded_clinear.clinear bounded_clinear_cblinfun_compose_right)
-
-lemma closure_of_eqI:
-  fixes f g :: \<open>'a \<Rightarrow> 'b\<close> and T :: \<open>'a topology\<close> and U :: \<open>'b topology\<close>
-  assumes haus: \<open>hausdorff U\<close>
-  assumes eq: \<open>\<And>x. x \<in> S \<Longrightarrow> f x = g x\<close>
-  assumes xS: \<open>x \<in> T closure_of S\<close>
-  assumes cont: \<open>continuous_map T U f\<close> \<open>continuous_map T U g\<close>
-  shows \<open>f x = g x\<close>
-    (* Like on_closure_eqI *)
-  thm on_closure_eqI
-  sorry
-
-(* lemma xxx: \<open>\<forall>\<^sub>\<tau> 's::chilbert_space = closure (cspan S) with (scaleR, scaleC, plus, 0, minus, uminus, dist, norm, sgn, uniformity, open, cinner). 
-          \<exists>B. B \<supseteq> S \<and> is_ortho_set B \<and> (\<forall>x\<in>B. norm x = 1) \<and> ccspan B = V\<close>
-  sorry
-thm xxx[cancel_with_type] *)
-
-lemma map_filter_on_id: \<open>map_filter_on S (\<lambda>x. x) F = F\<close> if \<open>\<forall>\<^sub>F x in F. x \<in> S\<close>
-  using that
-  by (auto intro!: filter_eq_iff[THEN iffD2] simp: eventually_map_filter_on eventually_frequently_simps)
-
-lemma inverse_real_inverse: \<open>inverse_real_inst.inverse_real = inverse\<close>
-  by (simp add: HOL.nitpick_unfold)
-
-named_theorems with_type_intros
-lemma [with_type_intros]: \<open>fst (A,B) \<noteq> {}\<close> if \<open>A \<noteq> {}\<close>
-  using that by simp
-lemma [with_type_intros]: \<open>with_type_compat_rel C (fst (S,p)) R\<close> if \<open>with_type_compat_rel C S R\<close>
-  using that by simp
-declare with_typeI[with_type_intros]
-
-lemma with_type_chilbert_space_class_subspaceI[with_type_intros]: \<open>fst with_type_chilbert_space_class
-     (fst (S, (*\<^sub>R), (*\<^sub>C), (+), 0, (-), uminus, dist, norm, sgn, uniformity_on S, openin (top_of_set S), (\<bullet>\<^sub>C)))
-     (snd (S, (*\<^sub>R), (*\<^sub>C), (+), 0, (-), uminus, dist, norm, sgn, uniformity_on S, openin (top_of_set S), (\<bullet>\<^sub>C)))\<close>
-  if [simp]: \<open>csubspace S\<close> \<open>closed S\<close>
-  (* TODO open and uniformity may need to be restricted! *)
-proof -
-  have open1: \<open>(\<exists>y. \<forall>x ya. rel_set (equal_onp S) x ya \<longrightarrow> open x = y ya)\<close>
-    apply (rule exI[of _ \<open>open\<close>])
-    by (smt (verit, ccfv_threshold) equal_onp_def rel_setD1 rel_setD2 subset_iff topological_space_class.openI)
-  have uniformity: \<open>rel_filter (rel_prod (equal_onp S) (equal_onp S)) (uniformity_on S) (uniformity_on S)\<close>
-    apply (rule rel_filter.intros[where Z=\<open>map_filter_on (S\<times>S) (\<lambda>x. (x,x)) (uniformity_on S)\<close>])
-      apply (simp add: eventually_map_filter_on always_eventually equal_onp_def eventually_inf_principal)
-     apply (subst map_filter_on_comp)
-    apply (auto simp add: map_filter_on_comp equal_onp_def eventually_inf_principal map_filter_on_id o_def)[3]
-     apply (subst map_filter_on_comp)
-    by (auto simp add: map_filter_on_comp equal_onp_def eventually_inf_principal map_filter_on_id o_def)
-  have 0: \<open>(\<exists>y. \<forall>x ya. rel_set (equal_onp S) x ya \<longrightarrow> openin (top_of_set S) x = y ya)\<close>
-    apply (rule exI[of _ \<open>openin (top_of_set S)\<close>])
-    by (metis equal_onp_def equalityI rel_setD1 rel_setD2 subset_iff)
-  have 1: \<open>with_type_chilbert_space_class_dom S ((*\<^sub>R), (*\<^sub>C), (+), 0, (-), uminus, dist, norm, sgn, uniformity_on S, openin (top_of_set S), (\<bullet>\<^sub>C))\<close>
-    apply (simp add: with_type_chilbert_space_class_dom_def Domainp_iff rel_fun_def equal_onp_def)
-    by (auto intro!: 0 exI uniformity simp add: scaleR_scaleC complex_vector.subspace_scale
-        complex_vector.subspace_add complex_vector.subspace_0 complex_vector.subspace_diff
-        complex_vector.subspace_neg sgn_div_norm open1)
-  have 2: \<open>with_type_chilbert_space_class_pred' (\<lambda>x. x \<in> S)
-     ((*\<^sub>R), (*\<^sub>C), (+), 0, (-), uminus, dist, norm, sgn, uniformity_on S, open, (\<bullet>\<^sub>C))\<close>
-    apply (simp add: with_type_chilbert_space_class_pred'_def scaleR_scaleC)
-    apply (intro conjI)
-               apply (auto simp add: complex_vector.vector_space_assms dist_norm sgn_div_norm scaleR_scaleC
-        cinner_simps inverse_real_inverse simp flip: of_real_inverse norm_eq_sqrt_cinner)
-            defer
-  defer
-  defer
-             defer
-             defer
-             defer
-    using norm_diff_triangle_le norm_imp_pos_and_ge norm_minus_commute apply blast
-
-    defer
-            defer
-    by -
-  from 1 2
-  show ?thesis
-    by (simp add: with_type_chilbert_space_class_def with_type_chilbert_space_class_pred_def)
-qed
-
-lemma orthonormal_subspace_basis_exists:
-  fixes S :: \<open>'a::chilbert_space set\<close>
-  assumes \<open>is_ortho_set S\<close> and \<open>\<And>x. x\<in>S \<Longrightarrow> norm x = 1\<close> and \<open>S \<subseteq> space_as_set V\<close>
-  shows \<open>\<exists>B. B \<supseteq> S \<and> is_ortho_set B \<and> (\<forall>x\<in>B. norm x = 1) \<and> ccspan B = V\<close>
-proof -
-  note [[show_hyps]]
-  (* TODO open and uniformity may need to be restricted! *)
-  have \<open>\<forall>\<^sub>\<tau> 's::chilbert_space = closure (cspan S) with (scaleR, scaleC, plus, 0, minus, uminus, dist, norm, sgn, uniformity, open, cinner). 
-          \<exists>B. B \<supseteq> S \<and> is_ortho_set B \<and> (\<forall>x\<in>B. norm x = 1) \<and> ccspan B = V\<close>
-  proof (intro with_type_intros)
-    show \<open>closure (cspan S) \<noteq> {}\<close>
-      using complex_vector.span_clauses(2) by auto
-    show \<open>csubspace (closure (cspan S))\<close>
-      using closure_is_csubspace by blast
-    show \<open>closed (closure (cspan S))\<close>
-      by simp
-    show \<open>with_type_compat_rel (fst with_type_chilbert_space_class)
-     (closure (cspan S)) (snd with_type_chilbert_space_class)\<close>
-      by (rule with_type_chilbert_space_class_rel_compat)
-    fix Rep :: \<open>'s \<Rightarrow> 'a\<close> and Abs abs_ops
-    assume \<open>type_definition Rep Abs
-        (fst (closure (cspan S), (*\<^sub>R), (*\<^sub>C), (+), 0, (-), uminus, dist, norm, sgn, uniformity, open, (\<bullet>\<^sub>C)))\<close>
-    then have \<open>type_definition Rep Abs (closure (cspan S))\<close>
-      by simp
-    assume \<open>snd with_type_chilbert_space_class (\<lambda>x y. x = Rep y)
-        (snd (closure (cspan S), (*\<^sub>R), (*\<^sub>C), (+), 0, (-), uminus, dist, norm, sgn, uniformity, open, (\<bullet>\<^sub>C))) abs_ops\<close>
-    then have \<open>with_type_chilbert_space_class_rel (\<lambda>x y. x = Rep y)
-        ((*\<^sub>R), (*\<^sub>C), (+), 0, (-), uminus, dist, norm, sgn, uniformity, open, (\<bullet>\<^sub>C)) abs_ops\<close>
-      unfolding with_type_chilbert_space_class_def
-      by simp
-    show \<open>\<exists>B. B \<supseteq> S \<and> is_ortho_set B \<and> (\<forall>x\<in>B. norm x = 1) \<and> ccspan B = V\<close>
-      apply transfer
-      thm orthonormal_basis_exists
-      by -
-  next show x for x by -
-  qed
-  from this[cancel_with_type]
-  show ?thesis
-    by simp
-qed
-
-(* TODO move *)
-lemma has_sum_in_comm_additive:
-  fixes f :: \<open>'a \<Rightarrow> 'b :: comm_monoid_add\<close>
-    and g :: \<open>'b \<Rightarrow> 'c :: comm_monoid_add\<close>
-  assumes \<open>continuous_map T U g\<close>
-  assumes \<open>\<And>x y. g (x+y) = g x + g y\<close>
-  assumes \<open>has_sum_in T f A l\<close>
-  shows \<open>has_sum_in U (g o f) A (g l)\<close>
-  sorry
-
-
-lemma infsum_butterfly_ket_a: \<open>has_sum_in weak_star_topology (\<lambda>i. butterfly (a *\<^sub>V ket i) (ket i)) UNIV a\<close>
-proof -
-  have \<open>has_sum_in weak_star_topology ((\<lambda>b. a o\<^sub>C\<^sub>L b) \<circ> (\<lambda>i. Misc.selfbutterket i)) UNIV (a o\<^sub>C\<^sub>L id_cblinfun)\<close>
-    apply (rule has_sum_in_comm_additive)
-    by (auto intro!: continuous_map_left_comp_weak_star infsum_butterfly_ket simp: cblinfun_compose_add_right)
-  then show ?thesis
-    by (auto simp: o_def cblinfun_comp_butterfly)
-qed
-
-
-lemma finite_rank_sum: \<open>finite_rank (\<Sum>x\<in>F. f x)\<close> if \<open>\<And>x. x\<in>F \<Longrightarrow> finite_rank (f x)\<close>
-  using that apply (induction F rule:infinite_finite_induct)
-  by (auto intro!: finite_rank_plus)
-
-lemma finite_rank_weak_star_dense[simp]: \<open>weak_star_topology closure_of (Collect finite_rank) = (UNIV :: ('a ell2 \<Rightarrow>\<^sub>C\<^sub>L 'b::chilbert_space) set)\<close>
-proof -
-  have \<open>x \<in> weak_star_topology closure_of (Collect finite_rank)\<close> for x :: \<open>'a ell2 \<Rightarrow>\<^sub>C\<^sub>L 'b\<close>
-  proof (rule limitin_closure_of)
-    define f :: \<open>'a \<Rightarrow> 'a ell2 \<Rightarrow>\<^sub>C\<^sub>L 'b\<close> where \<open>f = (\<lambda>i. butterfly (x *\<^sub>V ket i) (ket i))\<close>
-    have \<open>has_sum_in weak_star_topology f UNIV x\<close>
-      using f_def infsum_butterfly_ket_a by blast
-    then show \<open>limitin weak_star_topology (sum f) x (finite_subsets_at_top UNIV)\<close>
-      using has_sum_in_def by blast
-    show \<open>range (sum f) \<subseteq> Collect finite_rank\<close>
-      by (auto intro!: finite_rank_sum simp: f_def)
-    show \<open>finite_subsets_at_top UNIV \<noteq> \<bottom>\<close>
-      by simp
-  qed
-  then show ?thesis
-    by auto
-qed
-
-lemma trunc_ell2_singleton: \<open>trunc_ell2 {x} \<psi> = Rep_ell2 \<psi> x *\<^sub>C ket x\<close>
-  apply transfer by auto
-
-lemma trunc_ell2_insert: \<open>trunc_ell2 (insert x M) \<psi> = trunc_ell2 M \<psi> + Rep_ell2 \<psi> x *\<^sub>C ket x\<close> if \<open>x \<notin> M\<close>
-  using trunc_ell2_union_disjoint[where M=M and N=\<open>{x}\<close> and \<psi>=\<psi>]
-  using that by (auto simp: trunc_ell2_singleton)
-
-(* TODO move *)
-lemma trunc_ell2_finite_sum: \<open>trunc_ell2 M \<psi> = (\<Sum>i\<in>M. Rep_ell2 \<psi> i *\<^sub>C ket i)\<close> if \<open>finite M\<close>
-  using that apply induction by (auto simp: trunc_ell2_insert)
-
-(* TODO move *)
-lemma butterfly_sum_left: \<open>butterfly (\<Sum>i\<in>M. \<psi> i) \<phi> = (\<Sum>i\<in>M. butterfly (\<psi> i) \<phi>)\<close>
-  apply (induction M rule:infinite_finite_induct)
-  by (auto simp add: butterfly_add_left)
-
-(* TODO move *)
-lemma butterfly_sum_right: \<open>butterfly \<psi> (\<Sum>i\<in>M. \<phi> i) = (\<Sum>i\<in>M. butterfly \<psi> (\<phi> i))\<close>
-  apply (induction M rule:infinite_finite_induct)
-  by (auto simp add: butterfly_add_right)
-
-
-(* TODO move *)
-lemma finite_rank_dense_compact[simp]: \<open>closure (cspan {butterket \<xi> \<eta> |\<xi> \<eta>. True}) = Collect compact_op\<close>
-proof (rule Set.equalityI)
-  show \<open>closure (cspan {butterket \<xi> \<eta> |\<xi> \<eta>. True}) \<subseteq> Collect compact_op\<close>
-  proof -
-    have \<open>closure (cspan {butterket \<xi> \<eta> |\<xi> \<eta>. True}) \<subseteq> closure (Collect finite_rank)\<close>
-      apply (auto intro!: closure_mono simp: finite_rank_def)
-      by (smt (verit, del_insts) Collect_mono complex_vector.span_mono in_mono rank1_def)
-    also have \<open>\<dots> = Collect compact_op\<close>
-      by (simp add: Set.set_eqI compact_op_def)
-    finally show ?thesis
-      by -
-  qed
-  show \<open>Collect compact_op \<subseteq> closure (cspan {butterket \<xi> \<eta> |(\<xi>::'b) (\<eta>::'a). True})\<close>
-  proof -
-    have \<open>Collect compact_op = closure (cspan (Collect rank1))\<close>
-      by (metis compact_op_def finite_rank_def mem_Collect_eq subsetI subset_antisym)
-    also have \<open>\<dots> \<subseteq> closure (cspan (closure (cspan {butterket \<xi> \<eta> |(\<xi>::'b) (\<eta>::'a). True})))\<close>
-    proof (rule closure_mono, rule complex_vector.span_mono, rule subsetI)
-      fix x :: \<open>'a ell2 \<Rightarrow>\<^sub>C\<^sub>L 'b ell2\<close> assume \<open>x \<in> Collect rank1\<close>
-      then obtain a b where xab: \<open>x = butterfly a b\<close>
-        by (meson mem_Collect_eq rank1_def)
-      define f where \<open>f = (\<lambda>(F,G). butterfly (trunc_ell2 F a) (trunc_ell2 G b))\<close>
-      have lim: \<open>(f \<longlongrightarrow> x) (finite_subsets_at_top UNIV \<times>\<^sub>F finite_subsets_at_top UNIV)\<close>
-      proof (rule tendstoI, subst dist_norm)
-        fix e :: real assume \<open>e > 0\<close>
-        define d where \<open>d = (if norm a = 0 \<and> norm b = 0 then 1 else e / (max (norm a) (norm b)) / 4)\<close>
-        have d: \<open>norm a * d + norm a * d + norm b * d < e\<close>
-        proof -
-          have \<open>norm a * d \<le> e/4\<close>
-            using \<open>e > 0\<close> apply (auto simp: d_def)
-             apply (simp add: divide_le_eq)
-            by (smt (z3) Extra_Ordered_Fields.mult_sign_intros(3) \<open>0 < e\<close> antisym_conv divide_le_eq less_imp_le linordered_field_class.mult_imp_div_pos_le mult_left_mono nice_ordered_field_class.dense_le nice_ordered_field_class.divide_nonneg_neg nice_ordered_field_class.divide_nonpos_pos nle_le nonzero_mult_div_cancel_left norm_imp_pos_and_ge ordered_field_class.sign_simps(5) split_mult_pos_le)
-          moreover have \<open>norm b * d \<le> e/4\<close>
-            using \<open>e > 0\<close> apply (auto simp: d_def)
-             apply (simp add: divide_le_eq)
-            by (smt (verit) linordered_field_class.mult_imp_div_pos_le mult_left_mono norm_le_zero_iff ordered_field_class.sign_simps(5))
-          ultimately have \<open>norm a * d + norm a * d + norm b * d \<le> 3 * e / 4\<close>
-            by linarith
-          also have \<open>\<dots> < e\<close>
-            by (simp add: \<open>0 < e\<close>)
-          finally show ?thesis
-            by -
-        qed
-        have [simp]: \<open>d > 0\<close>
-          using \<open>e > 0\<close> apply (auto simp: d_def)
-           apply (smt (verit, best) nice_ordered_field_class.divide_pos_pos norm_eq_zero norm_not_less_zero)
-          by (smt (verit) linordered_field_class.divide_pos_pos zero_less_norm_iff)
-        from trunc_ell2_lim_at_UNIV[where \<psi>=a]
-        have \<open>\<forall>\<^sub>F F in finite_subsets_at_top UNIV. norm (trunc_ell2 F a - a) < d\<close>
-          by (metis Lim_null \<open>0 < d\<close> order_tendstoD(2) tendsto_norm_zero_iff)
-        moreover
-        from trunc_ell2_lim_at_UNIV[where \<psi>=b]
-        have \<open>\<forall>\<^sub>F G in finite_subsets_at_top UNIV. norm (trunc_ell2 G b - b) < d\<close>
-          by (metis Lim_null \<open>0 < d\<close> order_tendstoD(2) tendsto_norm_zero_iff)
-        ultimately have \<open>\<forall>\<^sub>F (F,G) in finite_subsets_at_top UNIV \<times>\<^sub>F finite_subsets_at_top UNIV. norm (trunc_ell2 F a - a) < d \<and> norm (trunc_ell2 G b - b) < d\<close>
-          unfolding case_prod_beta
-          by (rule eventually_prodI)
-        moreover have \<open>norm (f (F,G) - x) < e\<close> if \<open>norm (trunc_ell2 F a - a) < d\<close> and \<open>norm (trunc_ell2 G b - b) < d\<close> for F G
-        proof -
-          define B where \<open>B F G = butterfly (trunc_ell2 F a) (trunc_ell2 G b)\<close> for F G
-          have a_split: \<open>a = trunc_ell2 F a + trunc_ell2 (-F) a\<close>
-            by (simp add: Compl_eq_Diff_UNIV trunc_ell2_union_Diff)
-          have b_split: \<open>b = trunc_ell2 G b + trunc_ell2 (-G) b\<close>
-            by (simp add: Compl_eq_Diff_UNIV trunc_ell2_union_Diff)
-          have n1: \<open>norm (B F (-G)) \<le> norm a * d\<close> for F
-          proof -
-            have \<open>norm (B F (-G)) \<le> norm a * norm (trunc_ell2 (-G) b)\<close>
-              by (smt (verit, del_insts) B_def mult_right_mono norm_butterfly norm_ge_zero norm_id_minus_trunc_ell2 power2_eq_square square_less_square)
-            also have \<open>\<dots> \<le> norm a * norm (trunc_ell2 G b - b)\<close>
-              by (metis add_diff_cancel_left' b_split less_eq_real_def norm_minus_commute)
-            also have \<open>\<dots> \<le> norm a * d\<close>
-              by (meson less_eq_real_def mult_left_mono norm_ge_zero that(2))
-            finally show ?thesis
-              by -
-          qed
-          have n2: \<open>norm (B (-F) G) \<le> norm b * d\<close> for G
-          proof -
-            have \<open>norm (B (-F) G) \<le> norm b * norm (trunc_ell2 (-F) a)\<close>
-              apply (simp add: B_def norm_butterfly)
-              by (metis mult_right_mono norm_ge_zero ordered_field_class.sign_simps(33) top.extremum trunc_ell2_UNIV trunc_ell2_norm_mono)
-            also have \<open>\<dots> \<le> norm b * norm (trunc_ell2 F a - a)\<close>
-              by (smt (verit, best) a_split add_diff_cancel_left' minus_diff_eq norm_minus_cancel)
-            also have \<open>\<dots> \<le> norm b * d\<close>
-              by (meson less_eq_real_def mult_left_mono norm_ge_zero that(1))
-            finally show ?thesis
-              by -
-          qed
-          have \<open>norm (f (F,G) - x) = norm (B F G - butterfly a b)\<close>
-            by (simp add: f_def xab B_def)
-          also have \<open>\<dots> = norm (- B F (-G) - B (-F) (-G) - B (-F) G)\<close>
-            apply (subst a_split, subst b_split)
-            by (simp add: B_def butterfly_add_right butterfly_add_left)
-          also have \<open>\<dots> \<le> norm (B F (-G)) + norm (B (-F) (-G)) + norm (B (-F) G)\<close>
-            by (smt (verit, best) norm_minus_cancel norm_triangle_ineq4)
-          also have \<open>\<dots> \<le> norm a * d + norm a * d + norm b * d\<close>
-            using n1 n2
-            by (meson add_mono_thms_linordered_semiring(1))
-          also have \<open>\<dots> < e\<close>
-            by (fact d)
-          finally show ?thesis
-            by -
-        qed
-        ultimately show \<open>\<forall>\<^sub>F FG in finite_subsets_at_top UNIV \<times>\<^sub>F finite_subsets_at_top UNIV. norm (f FG - x) < e\<close>
-          by (smt (verit, ccfv_SIG) eventually_mono f_def prod.case_eq_if split_conv)
-      qed
-      have nontriv: \<open>finite_subsets_at_top UNIV \<times>\<^sub>F finite_subsets_at_top UNIV \<noteq> \<bottom>\<close>
-        by (simp add: prod_filter_eq_bot)
-      have inside: \<open>\<forall>\<^sub>F x in finite_subsets_at_top UNIV \<times>\<^sub>F finite_subsets_at_top UNIV. f x \<in> cspan {butterket \<xi> \<eta> |\<xi> \<eta>. True}\<close>
-      proof (rule eventually_mp[where P=\<open>\<lambda>(F,G). finite F \<and> finite G\<close>])
-        show \<open>\<forall>\<^sub>F (F,G) in finite_subsets_at_top UNIV \<times>\<^sub>F finite_subsets_at_top UNIV. finite F \<and> finite G\<close>
-          by (smt (verit) case_prod_conv eventually_finite_subsets_at_top_weakI eventually_prod_filter)
-        have \<open>f (F,G) \<in> cspan {butterket \<xi> \<eta> |\<xi> \<eta>. True}\<close> if [simp]: \<open>finite F\<close> \<open>finite G\<close> for F G
-          by (auto intro!: complex_vector.span_sum complex_vector.span_scale complex_vector.span_base[where a=\<open>butterfly _ _\<close>]
-              simp add: f_def trunc_ell2_finite_sum butterfly_sum_left butterfly_sum_right)
-        then show \<open>\<forall>\<^sub>F x in finite_subsets_at_top UNIV \<times>\<^sub>F finite_subsets_at_top UNIV. (case x of (F, G) \<Rightarrow> finite F \<and> finite G) \<longrightarrow> f x \<in> cspan {Misc.butterket \<xi> \<eta> |\<xi> \<eta>. True}\<close>
-          apply auto
-          by (simp add: always_eventually)
-      qed
-      show \<open>x \<in> closure (cspan {butterket \<xi> \<eta> |\<xi> \<eta>. True})\<close>
-        using lim nontriv inside by (rule limit_in_closure)
-    qed
-    also have \<open>\<dots> = closure (cspan {butterket \<xi> \<eta> |(\<xi>::'b) (\<eta>::'a). True})\<close>
-      by (simp add: complex_vector.span_eq_iff[THEN iffD2])
-    finally show ?thesis
-      by -
-  qed
-qed
-
-(* TODO move *)
-lemma butterkets_weak_star_dense[simp]:
-  \<open>weak_star_topology closure_of cspan {butterket (\<xi>::'a) (\<eta>::'b) |\<xi> \<eta>. True} = UNIV\<close>
-proof -
-  from continuous_map_image_closure_subset[OF weak_star_topology_weaker_than_euclidean]
-  have \<open>weak_star_topology closure_of (cspan {butterket (\<xi>::'a) (\<eta>::'b) |\<xi> \<eta>. True}) \<supseteq> closure (cspan {butterket \<xi> \<eta> |\<xi> \<eta>. True})\<close> (is \<open>_ \<supseteq> \<dots>\<close>)
-    by auto
-  moreover from finite_rank_dense_compact
-  have \<open>\<dots> \<supseteq> Collect finite_rank\<close>
-    by (metis closure_subset compact_op_def mem_Collect_eq subsetI subset_antisym)
-  ultimately have *: \<open>weak_star_topology closure_of (cspan {butterket (\<xi>::'a) (\<eta>::'b) |\<xi> \<eta>. True}) \<supseteq> Collect finite_rank\<close>
-    by simp
-  have \<open>weak_star_topology closure_of cspan {butterket \<xi> \<eta> |\<xi> \<eta>. True}
-        = weak_star_topology closure_of (weak_star_topology closure_of cspan {butterket (\<xi>::'a) (\<eta>::'b) |\<xi> \<eta>. True})\<close>
-  by simp
-  also have \<open>\<dots> \<supseteq> weak_star_topology closure_of Collect finite_rank\<close> (is \<open>_ \<supseteq> \<dots>\<close>)
-    using * closure_of_mono by blast
-  also have \<open>\<dots> = UNIV\<close>
-    by simp
-  finally show ?thesis
-    by auto
-qed
-
-lemma sandwich_weak_star_cont[simp]:
-  \<open>continuous_map weak_star_topology weak_star_topology (sandwich A)\<close>
-  using continuous_map_compose[OF continuous_map_left_comp_weak_star continuous_map_right_comp_weak_star]
-  by (auto simp: o_def sandwich_def[abs_def])
-
-(* lemma continuous_map_cong:
-  assumes \<open>\<And>x. x \<in> topspace T \<Longrightarrow> f x = g x\<close>
-  shows \<open>continuous_map T S f \<longleftrightarrow> continuous_map T S g\<close>
-  by (metis assms continuous_map_eq)
- *)
-
-(* 
-definition infsumopt where \<open>infsumopt f A = (if f summable_on A then Some (infsum f A) else None)\<close>
-
-syntax (ASCII)
-  "_infsumopt" :: "pttrn \<Rightarrow> 'a set \<Rightarrow> 'b \<Rightarrow> 'b::topological_comm_monoid_add option"  ("(3INFSUM? (_/:_)./ _)" [0, 51, 10] 10)
-syntax
-  "_infsumopt" :: "pttrn \<Rightarrow> 'a set \<Rightarrow> 'b \<Rightarrow> 'b::topological_comm_monoid_add option"  ("(2\<Sum>\<^sub>\<infinity>\<^sub>?(_/\<in>_)./ _)" [0, 51, 10] 10)
-translations \<comment> \<open>Beware of argument permutation!\<close>
-  "\<Sum>\<^sub>\<infinity>\<^sub>?i\<in>A. b" \<rightleftharpoons> "CONST infsumopt (\<lambda>i. b) A"
-
-syntax (ASCII)
-  "_univinfsumopt" :: "pttrn \<Rightarrow> 'a \<Rightarrow> 'a option"  ("(3INFSUM? _./ _)" [0, 10] 10)
-syntax
-  "_univinfsumopt" :: "pttrn \<Rightarrow> 'a \<Rightarrow> 'a option"  ("(2\<Sum>\<^sub>\<infinity>\<^sub>?_./ _)" [0, 10] 10)
-translations
-  "\<Sum>\<^sub>\<infinity>\<^sub>?x. t" \<rightleftharpoons> "CONST infsumopt (\<lambda>x. t) (CONST UNIV)"
- *)
-
-ML \<open>
-type lifted_typ = Type.
-
-
-type env = (bool * typ) list
-fun lift_term_to_maybe (env:env) (Bound i) : (bool * typ * term) = let val (lifted, typ) = nth env i in (lifted, typ, Bound i) end
-  | lift_term_to_maybe env (Const(\<^const_name>\<open>divide\<close>, _)
-\<close>
-    
-
-lemma TODO_NAME: \<open>trace (partial_trace' t o\<^sub>C\<^sub>L x) = trace (t o\<^sub>C\<^sub>L (x \<otimes>\<^sub>o id_cblinfun))\<close> if \<open>trace_class t\<close>
-  sorry
-
-lemma sandwich_weak_star_cont[simp]:
-  \<open>continuous_map weak_star_topology weak_star_topology (sandwich A)\<close>
-  using continuous_map_compose[OF continuous_map_left_comp_weak_star continuous_map_right_comp_weak_star]
-  by (auto simp: o_def sandwich_def[abs_def])
-
-(* lemma continuous_map_cong:
-  assumes \<open>\<And>x. x \<in> topspace T \<Longrightarrow> f x = g x\<close>
-  shows \<open>continuous_map T S f \<longleftrightarrow> continuous_map T S g\<close>
-sledgehammer
-  by (metis assms continuous_map_eq)
-sorry
- *)
-
-lemma continuous_map_pullback_both:
-  assumes cont: \<open>continuous_map T1 T2 g'\<close>
-  assumes g'g: \<open>\<And>x. f1 x \<in> topspace T1 \<and> x \<in> A1 \<Longrightarrow> g' (f1 x) = f2 (g x)\<close>
-  assumes top1: \<open>f1 -` topspace T1 \<inter> A1 \<subseteq> g -` A2\<close>
-  shows \<open>continuous_map (pullback_topology A1 f1 T1) (pullback_topology A2 f2 T2) g\<close>
-proof -
-  from cont
-  have \<open>continuous_map (pullback_topology A1 f1 T1) T2 (g' \<circ> f1)\<close>
-    by (rule continuous_map_pullback)
-  then have \<open>continuous_map (pullback_topology A1 f1 T1) T2 (f2 \<circ> g)\<close>
-    apply (rule continuous_map_eq)
-    by (simp add: g'g topspace_pullback_topology)
-  then show ?thesis
-    apply (rule continuous_map_pullback')
-    by (simp add: top1 topspace_pullback_topology)
-qed
-
-definition partial_trace :: \<open>(('a \<times> 'c) ell2 \<Rightarrow>\<^sub>C\<^sub>L ('b \<times> 'c) ell2)  \<Rightarrow> ('a ell2 \<Rightarrow>\<^sub>C\<^sub>L 'b ell2)\<close> where
-  \<open>partial_trace t = (\<Sum>\<^sub>\<infinity>j. (tensor_ell2_right (ket j))* o\<^sub>C\<^sub>L t o\<^sub>C\<^sub>L (tensor_ell2_right (ket j)))\<close>
-
-lemma  
-  assumes \<open>trace_class t\<close>
-  shows partial_trace_has_sum: \<open>has_sum (\<lambda>j. (tensor_ell2_right (ket j))* o\<^sub>C\<^sub>L t o\<^sub>C\<^sub>L (tensor_ell2_right (ket j))) UNIV (partial_trace t)\<close>
-  and partial_trace_summable: \<open>(\<lambda>j. (tensor_ell2_right (ket j))* o\<^sub>C\<^sub>L t o\<^sub>C\<^sub>L (tensor_ell2_right (ket j))) abs_summable_on UNIV\<close>
-proof -
-  show \<open>(\<lambda>j. (tensor_ell2_right (ket j))* o\<^sub>C\<^sub>L t o\<^sub>C\<^sub>L (tensor_ell2_right (ket j))) abs_summable_on UNIV\<close>
-    by -
-  then show \<open>has_sum (\<lambda>j. (tensor_ell2_right (ket j))* o\<^sub>C\<^sub>L t o\<^sub>C\<^sub>L (tensor_ell2_right (ket j))) UNIV (partial_trace t)\<close>
-    by (simp add: Axioms_Complement_Quantum.partial_trace_def abs_summable_summable)
-qed
-
-lemma partial_trace_trace_class[simp]: \<open>trace_class (partial_trace t)\<close> if \<open>trace_class t\<close>
-proof -
-  have \<open>(\<lambda>x. x \<bullet>\<^sub>C (abs_op (partial_trace t) *\<^sub>V x)) abs_summable_on range ket\<close>
-    by -
-  then show \<open>trace_class (partial_trace t)\<close>
-    using is_onb_ket
-    by (rule trace_classI[rotated])
-qed
-
-lemma TODO_NAME2: \<open>trace (partial_trace t o\<^sub>C\<^sub>L x) = trace (t o\<^sub>C\<^sub>L (x \<otimes>\<^sub>o id_cblinfun))\<close> if \<open>trace_class t\<close>
-  sorry
-
-(* TODO move *)
-lemma amplification_weak_star_cont[simp]:
-  \<open>continuous_map weak_star_topology weak_star_topology (\<lambda>a. a \<otimes>\<^sub>o id_cblinfun)\<close>
-(* Two proofs (due to merge), I think first is more current. *)
-  sorry
-(*
-proof (unfold weak_star_topology_def, rule continuous_map_pullback_both)
-  define g' :: \<open>('b ell2 \<Rightarrow>\<^sub>C\<^sub>L 'a ell2 \<Rightarrow> complex)
-   \<Rightarrow> ('b \<times> 'c) ell2 \<Rightarrow>\<^sub>C\<^sub>L ('a \<times> 'c) ell2 \<Rightarrow> complex\<close> where \<open>g' \<tau> t = \<tau> (if trace_class t then partial_trace t else 0)\<close> for \<tau> t
-  have \<open>continuous_on UNIV g'\<close>
-    by (simp add: continuous_on_coordinatewise_then_product g'_def)
-  then show \<open>continuous_map euclidean euclidean g'\<close>
-    using continuous_map_iff_continuous2 by blast
-  show \<open>g' (\<lambda>t. if trace_class t then trace (t o\<^sub>C\<^sub>L x) else 0) =
-         (\<lambda>t. if trace_class t then trace (t o\<^sub>C\<^sub>L x \<otimes>\<^sub>o id_cblinfun) else 0)\<close> for x
-    by (auto intro!: ext simp: g'_def TODO_NAME2) 
-qed auto
- *)
-(*
-proof (unfold weak_star_topology_def', rule continuous_map_pullback_both)
-  define g' :: \<open>(('b ell2, 'a ell2) trace_class \<Rightarrow> complex) \<Rightarrow> (('b \<times> 'c) ell2, ('a \<times> 'c) ell2) trace_class \<Rightarrow> complex\<close> where
-    \<open>g' \<tau> t = \<tau> (partial_trace t)\<close> for \<tau> t
-  have \<open>continuous_on UNIV g'\<close>
-    by (simp add: continuous_on_coordinatewise_then_product g'_def)
-  then show \<open>continuous_map euclidean euclidean g'\<close>
-    using continuous_map_iff_continuous2 by blast
-  show \<open>g' (\<lambda>t. trace (from_trace_class t o\<^sub>C\<^sub>L x)) = (\<lambda>t. trace (from_trace_class t o\<^sub>C\<^sub>L x \<otimes>\<^sub>o id_cblinfun))\<close> for x
-    by (auto intro!: ext simp: g'_def TODO_NAME) 
-qed auto
- *)
 
 lemma register_decomposition:
-  fixes \<Phi> :: \<open>'a update \<Rightarrow> 'b update\<close>
+  fixes \<Phi> :: \<open>'a::finite update \<Rightarrow> 'b::finite update\<close>
   assumes [simp]: \<open>register \<Phi>\<close>
-  shows \<open>\<forall>\<^sub>\<tau> 'c::type = register_decomposition_basis \<Phi>.
-         (\<exists>U :: ('a \<times> 'c) ell2 \<Rightarrow>\<^sub>C\<^sub>L 'b ell2. unitary U \<and> 
-              (\<forall>\<theta>. \<Phi> \<theta> = sandwich U (\<theta> \<otimes>\<^sub>o id_cblinfun)))\<close>
+  shows \<open>\<exists>U :: ('a \<times> ('a, 'b) complement_domain) ell2 \<Rightarrow>\<^sub>C\<^sub>L 'b ell2. unitary U \<and> 
+              (\<forall>\<theta>. \<Phi> \<theta> = sandwich U (\<theta> \<otimes>\<^sub>o id_cblinfun))\<close>
   \<comment> \<open>Proof based on @{cite daws21unitalanswer}\<close>
-proof (rule with_typeI; unfold fst_conv snd_conv)
-  show \<open>fst with_type_type_class (register_decomposition_basis \<Phi>) ()\<close>
-    by (simp add: with_type_type_class_def)
-  show \<open>with_type_compat_rel (fst with_type_type_class) (register_decomposition_basis \<Phi>) (snd with_type_type_class)\<close>
-    using with_type_compat_rel_type by blast
-
+proof -
   note [[simproc del: compatibility_warn]]
-  define \<xi>0 :: 'a where \<open>\<xi>0 = undefined\<close>
+  fix \<xi>0 :: 'a
 
-  have \<open>bounded_clinear \<Phi>\<close>
-    using assms register_def by blast
-  then have [simp]: \<open>clinear \<Phi>\<close>
-    by (simp add: bounded_clinear.clinear)
+  have [simp]: \<open>clinear \<Phi>\<close>
+    by simp
 
-  define P where \<open>P i = selfbutterket i\<close> for i :: 'a
-
-  note blinfun_cblinfun_eq_bi_unique[transfer_rule del]
-  note cblinfun.bi_unique[transfer_rule del]
-  note cblinfun.left_unique[transfer_rule del]
-  note cblinfun.right_unique[transfer_rule del]
-  note cblinfun.right_total[transfer_rule del]
-  note id_cblinfun.transfer[transfer_rule del]
+  define P where \<open>P i = Proj (ccspan {ket i})\<close> for i :: 'a
+  have P_butter: \<open>P i = selfbutterket i\<close> for i
+    by (simp add: P_def butterfly_eq_proj)
 
   define P' where \<open>P' i = \<Phi> (P i)\<close> for i :: 'a
   have proj_P': \<open>is_Proj (P' i)\<close> for i
-    by (simp add: P_def P'_def butterfly_is_Proj register_projector)
-  have sumP'id2: \<open>has_sum_in weak_star_topology (\<lambda>i. P' i) UNIV id_cblinfun\<close> (* TODO: we use this one *)
-  proof -
-    from infsum_butterfly_ket
-    have \<open>has_sum_in weak_star_topology (\<Phi> o selfbutterket) UNIV (\<Phi> id_cblinfun)\<close>
-      apply (rule has_sum_in_comm_additive[rotated -1])
-      using assms by (auto simp: complex_vector.linear_add register_def)
-    then show ?thesis
-      by (simp add: P'_def P_def o_def)
-  qed
+    by (simp add: P_def P'_def register_projector)
+  have \<open>(\<Sum>i\<in>UNIV. P i) = id_cblinfun\<close>
+    using sum_butterfly_ket P_butter by simp
+  then have sumP'id: \<open>(\<Sum>i\<in>UNIV. P' i) = id_cblinfun\<close>
+    unfolding P'_def 
+    apply (subst complex_vector.linear_sum[OF \<open>clinear \<Phi>\<close>, symmetric])
+    by auto
 
   define S where \<open>S i = P' i *\<^sub>S \<top>\<close> for i :: 'a
   have P'id: \<open>P' i *\<^sub>V \<psi> = \<psi>\<close> if \<open>\<psi> \<in> space_as_set (S i)\<close> for i \<psi>
     using S_def that proj_P'
     by (metis cblinfun_fixes_range is_Proj_algebraic)
 
-  define S_iso' :: \<open>'a \<Rightarrow> 'a \<Rightarrow> 'a update\<close> where \<open>S_iso' i j = classical_operator (Some o Transposition.transpose i j)\<close> for i j :: 'a
-  have S_iso'_apply: \<open>S_iso' i j *\<^sub>V ket i = ket j\<close> for i j
-    by (simp add: S_iso'_def classical_operator_ket classical_operator_exists_inj)
-  have S_iso'_unitary: \<open>unitary (S_iso' i j)\<close> for i j
-    by (simp add: S_iso'_def unitary_classical_operator)
-  have S_iso'_id: \<open>S_iso' i i = id_cblinfun\<close> for i
-    by (auto intro!: equal_ket simp: S_iso'_def classical_operator_ket classical_operator_exists_inj)
-  have S_iso'_adj_apply: \<open>(S_iso' i j)* *\<^sub>V ket j = ket i\<close> for i j
-    by (metis S_iso'_apply S_iso'_unitary cblinfun_apply_cblinfun_compose id_cblinfun_apply unitaryD1)
-  define S_iso where \<open>S_iso i j = \<Phi> (S_iso' i j)\<close> for i j
-  have uni_S_iso: \<open>unitary (S_iso i j)\<close> for i j
-    by (simp add: S_iso_def S_iso'_unitary register_unitary)
-  have S_iso_S: \<open>S_iso i j *\<^sub>S S i = S j\<close> for i j
-  proof -
-    have \<open>S_iso i j *\<^sub>S S i = S_iso i j *\<^sub>S P' i *\<^sub>S S_iso j i *\<^sub>S \<top>\<close>
-      by (simp add: S_def uni_S_iso)
-    also have \<open>\<dots> = S j\<close>
-      by (simp add: S_def P'_def S_iso_def P_def register_mult butterfly_comp_cblinfun cblinfun_comp_butterfly S_iso'_apply S_iso'_adj_apply
-        flip: cblinfun_compose_image)
-    finally show ?thesis
-      by -
-  qed
-  have S_iso_id[simp]: \<open>S_iso i i = id_cblinfun\<close> for i
-    by (simp add: S_iso'_id S_iso_def)
+  obtain B0 where finiteB0: \<open>finite (B0 i)\<close> and cspanB0: \<open>cspan (B0 i) = space_as_set (S i)\<close> for i
+    apply atomize_elim apply (simp flip: all_conj_distrib) apply (rule choice)
+    by (meson cfinite_dim_finite_subspace_basis csubspace_space_as_set)
 
-  obtain B\<^sub>0 where B\<^sub>0: \<open>is_ortho_set B\<^sub>0\<close> \<open>\<And>b. b \<in> B\<^sub>0 \<Longrightarrow> norm b = 1\<close> \<open>ccspan B\<^sub>0 = S \<xi>0\<close>
-    using orthonormal_subspace_basis_exists[where S="{}" and V=\<open>S \<xi>0\<close>]
-    apply atomize_elim by auto
+  obtain B where orthoB: \<open>is_ortho_set (B i)\<close>
+    and normalB: \<open>\<And>b. b \<in> B i \<Longrightarrow> norm b = 1\<close>
+    and cspanB: \<open>cspan (B i) = cspan (B0 i)\<close>
+    and finiteB: \<open>finite (B i)\<close> for i
+    apply atomize_elim apply (simp flip: all_conj_distrib) apply (rule choice)
+    using orthonormal_basis_of_cspan[OF finiteB0] by blast
 
-  have register_decomposition_basis_\<Phi>: \<open>is_ortho_set (register_decomposition_basis \<Phi>) \<and>
-       (\<forall>b\<in>register_decomposition_basis \<Phi>. norm b = 1) \<and>
-       ccspan (register_decomposition_basis \<Phi>) = S \<xi>0\<close>
-    unfolding register_decomposition_basis_def
-    apply (rule someI2[where a=B\<^sub>0])
-    using B\<^sub>0 by (auto simp: S_def P'_def P_def \<xi>0_def)
-
-  define B where \<open>B i = S_iso \<xi>0 i ` register_decomposition_basis \<Phi>\<close> for i
-  have B\<xi>0: \<open>B \<xi>0 = register_decomposition_basis \<Phi>\<close>
-    using B_def by force
-  have orthoB: \<open>is_ortho_set (B i)\<close> for i
-    apply (auto simp add: B_def is_ortho_set_def)
-    apply (metis (no_types, lifting) register_decomposition_basis_\<Phi> UNIV_I cblinfun_apply_cblinfun_compose cblinfun_fixes_range cinner_adj_left id_cblinfun_adjoint is_ortho_set_def top_ccsubspace.rep_eq uni_S_iso unitaryD1 unitary_id unitary_range)
-    by (metis register_decomposition_basis_\<Phi> cinner_ket_same cinner_zero_left cnorm_eq_1 isometry_preserves_norm orthogonal_ket uni_S_iso unitary_isometry)
-  have normalB: \<open>\<And>b. b \<in> B i \<Longrightarrow> norm b = 1\<close> for i
-    by (metis (no_types, lifting) register_decomposition_basis_\<Phi> B_def imageE isometry_preserves_norm uni_S_iso unitary_twosided_isometry)
-  have cspanB: \<open>ccspan (B i) = S i\<close> for i
-    by (simp add: B_def register_decomposition_basis_\<Phi> B\<xi>0 S_iso_S flip: cblinfun_image_ccspan)
-
+  from cspanB cspanB0 have cspanB: \<open>cspan (B i) = space_as_set (S i)\<close> for i
+    by simp
+  then have ccspanB: \<open>ccspan (B i) = S i\<close> for i
+    by (metis ccspan.rep_eq closure_finite_cspan finiteB space_as_set_inject)
   from orthoB have indepB: \<open>cindependent (B i)\<close> for i
     by (simp add: Complex_Inner_Product.is_ortho_set_cindependent)
 
   have orthoBiBj: \<open>is_orthogonal x y\<close> if \<open>x \<in> B i\<close> and \<open>y \<in> B j\<close> and \<open>i \<noteq> j\<close> for x y i j
   proof -
-    have \<open>P' i o\<^sub>C\<^sub>L P' j = 0\<close>
-      using \<open>i \<noteq> j\<close>
-      by (simp add: P'_def P_def register_mult butterfly_comp_butterfly cinner_ket
-          \<open>clinear \<Phi>\<close> complex_vector.linear_0)
-    then have *: \<open>Proj (ccspan (B i)) o\<^sub>C\<^sub>L Proj (ccspan (B j)) = 0\<close>
-      by (simp add: Proj_on_own_range S_def cspanB proj_P')
-    then show \<open>is_orthogonal x y\<close>
-      by (meson orthogonal_projectors_orthogonal_spaces that(1) that(2))
+    from \<open>x \<in> B i\<close> obtain x' where x: \<open>x = P' i *\<^sub>V x'\<close>
+      by (metis S_def cblinfun_fixes_range complex_vector.span_base cspanB is_Proj_idempotent proj_P')
+    from \<open>y \<in> B j\<close> obtain y' where y: \<open>y = P' j *\<^sub>V y'\<close>
+      by (metis S_def cblinfun_fixes_range complex_vector.span_base cspanB is_Proj_idempotent proj_P')
+    have \<open>cinner x y = cinner (P' i *\<^sub>V x') (P' j *\<^sub>V  y')\<close>
+      using x y by simp
+    also have \<open>\<dots> = cinner (P' j *\<^sub>V P' i *\<^sub>V x') y'\<close>
+      by (metis cinner_adj_left is_Proj_algebraic proj_P')
+    also have \<open>\<dots> = cinner (\<Phi> (P j o\<^sub>C\<^sub>L P i) *\<^sub>V x') y'\<close>
+      unfolding P'_def register_mult[OF \<open>register \<Phi>\<close>, symmetric] by simp
+    also have \<open>\<dots> = cinner (\<Phi> (selfbutterket j o\<^sub>C\<^sub>L selfbutterket i) *\<^sub>V x') y'\<close>
+      unfolding P_butter by simp
+    also have \<open>\<dots> = cinner (\<Phi> 0 *\<^sub>V x') y'\<close>
+      by (metis butterfly_comp_butterfly complex_vector.scale_eq_0_iff orthogonal_ket that(3))
+    also have \<open>\<dots> = 0\<close>
+      by (simp add: complex_vector.linear_0)
+    finally show ?thesis
+      by -
   qed
+
 
   define B' where \<open>B' = (\<Union>i\<in>UNIV. B i)\<close>
 
   have P'B: \<open>P' i = Proj (ccspan (B i))\<close> for i
-    unfolding cspanB S_def
+    unfolding ccspanB S_def
     using proj_P' Proj_on_own_range'[symmetric] is_Proj_algebraic by blast
 
-  show \<open>register_decomposition_basis \<Phi> \<noteq> {}\<close>
-  proof (rule ccontr, simp)
-    assume \<open>register_decomposition_basis \<Phi> = {}\<close>
-    then have \<open>B i = {}\<close> for i
-      by (simp add: B_def)
-    then have \<open>S i = 0\<close> for i
-      using cspanB by force
-    then have \<open>P' i = 0\<close> for i
-      by (simp add: P'B cspanB)
-    with sumP'id2
-    have \<open>has_sum_in weak_star_topology (\<lambda>i. 0) UNIV id_cblinfun\<close>
-      by (metis (no_types, lifting) UNIV_I has_sum_in_0 has_sum_in_cong has_sum_in_unique hausdorff_weak_star id_cblinfun_not_0 weak_star_topology_topspace)
-    then have \<open>id_cblinfun = 0\<close>
-      using has_sum_in_0 has_sum_in_unique hausdorff_weak_star id_cblinfun_not_0 weak_star_topology_topspace by fastforce
-    then show False
-      using id_cblinfun_not_0 by blast
+  have \<open>(\<Sum>i\<in>UNIV. P' i) = Proj (ccspan B')\<close>
+  proof (unfold B'_def, use finite[of UNIV] in induction)
+    case empty
+    show ?case by auto
+  next
+    case (insert j M)
+    have \<open>(\<Sum>i\<in>insert j M. P' i) = P' j + (\<Sum>i\<in>M. P' i)\<close>
+      by (meson insert.hyps(1) insert.hyps(2) sum.insert)
+    also have \<open>\<dots> = Proj (ccspan (B j)) + Proj (ccspan (\<Union>i\<in>M. B i))\<close>
+      unfolding P'B insert.IH[symmetric] by simp
+    also have \<open>\<dots> = Proj (ccspan (B j \<union> (\<Union>i\<in>M. B i)))\<close>
+      apply (rule Proj_orthog_ccspan_union[symmetric])
+      using orthoBiBj insert.hyps(2) by auto
+    also have \<open>\<dots> = Proj (ccspan (\<Union>i\<in>insert j M. B i))\<close>
+      by auto
+    finally show ?case
+      by simp
   qed
+
+  with sumP'id 
+  have ccspanB': \<open>ccspan B' = \<top>\<close>
+    by (metis Proj_range cblinfun_image_id)
+  hence cspanB': \<open>cspan B' = UNIV\<close>
+    by (metis B'_def finiteB ccspan.rep_eq finite_UN_I finite_class.finite_UNIV closure_finite_cspan top_ccsubspace.rep_eq)
 
   from orthoBiBj orthoB have orthoB': \<open>is_ortho_set B'\<close>
     unfolding B'_def is_ortho_set_def by blast
   then have indepB': \<open>cindependent B'\<close>
     using is_ortho_set_cindependent by blast
+  have cardB': \<open>card B' = CARD('b)\<close>
+    apply (subst complex_vector.dim_span_eq_card_independent[symmetric])
+     apply (rule indepB')
+    apply (subst cspanB')
+    using cdim_UNIV_ell2 by auto
 
   from orthoBiBj orthoB
   have Bdisj: \<open>B i \<inter> B j = {}\<close> if \<open>i \<noteq> j\<close> for i j
     unfolding is_ortho_set_def
     apply auto by (metis cinner_eq_zero_iff that)
 
-  fix rep_c :: \<open>'c \<Rightarrow> 'b ell2\<close> and abs_c
-  assume typedef_c: \<open>type_definition rep_c abs_c (register_decomposition_basis \<Phi>)\<close>
-  then interpret type_definition rep_c abs_c \<open>register_decomposition_basis \<Phi>\<close> .
+  have cardBsame: \<open>card (B i) = card (B j)\<close> for i j
+  proof -
+    define Si_to_Sj where \<open>Si_to_Sj i j \<psi> = \<Phi> (butterket j i) *\<^sub>V \<psi>\<close> for i j \<psi>
+    have S2S2S: \<open>Si_to_Sj j i (Si_to_Sj i j \<psi>) = \<psi>\<close> if \<open>\<psi> \<in> space_as_set (S i)\<close> for i j \<psi>
+      using that P'id
+      by (simp add: Si_to_Sj_def cblinfun_apply_cblinfun_compose[symmetric] register_mult P_butter P'_def)
+    also have lin[simp]: \<open>clinear (Si_to_Sj i j)\<close> for i j
+      unfolding Si_to_Sj_def by simp
+    have S2S: \<open>Si_to_Sj i j x \<in> space_as_set (S j)\<close> for i j x
+    proof -
+      have \<open>Si_to_Sj i j x = P' j *\<^sub>V Si_to_Sj i j x\<close>
+        by (simp add: Si_to_Sj_def cblinfun_apply_cblinfun_compose[symmetric] register_mult P_butter P'_def)
+      also have \<open>P' j *\<^sub>V Si_to_Sj i j x \<in> space_as_set (S j)\<close>
+        by (simp add: S_def)
+      finally show ?thesis by -
+    qed
+    have bij: \<open>bij_betw (Si_to_Sj i j) (space_as_set (S i)) (space_as_set (S j))\<close>
+      apply (rule bij_betwI[where g=\<open>Si_to_Sj j i\<close>])
+      using S2S S2S2S by (auto intro!: funcsetI)
+    have \<open>cdim (space_as_set (S i)) = cdim (space_as_set (S j))\<close>
+      using lin apply (rule isomorphic_equal_cdim[where f=\<open>Si_to_Sj i j\<close>])
+      using bij apply (auto simp: bij_betw_def)
+      by (metis complex_vector.span_span cspanB)
+    then show ?thesis
+      by (metis complex_vector.dim_span_eq_card_independent cspanB indepB)
+  qed
 
-  have bij_rep_c: \<open>bij_betw rep_c (UNIV :: 'c set) (B \<xi>0)\<close>
-    unfolding B\<xi>0
-    apply (rule bij_betwI[where g=abs_c])
-    using Rep Rep_inverse Abs_inverse by blast+
+  have CARD'b: \<open>CARD('b) = card (B \<xi>0) * CARD('a)\<close>
+  proof -
+    have \<open>CARD('b) = card B'\<close>
+      using cardB' by simp
+    also have \<open>\<dots> = (\<Sum>i\<in>UNIV. card (B i))\<close>
+      unfolding B'_def apply (rule card_UN_disjoint)
+      using finiteB Bdisj by auto
+    also have \<open>\<dots> = (\<Sum>(i::'a)\<in>UNIV. card (B \<xi>0))\<close>
+      using cardBsame by metis
+    also have \<open>\<dots> = card (B \<xi>0) * CARD('a)\<close>
+      by auto
+    finally show ?thesis by -
+  qed
 
-  define u where \<open>u = (\<lambda>(\<xi>,\<alpha>). \<Phi> (butterket \<xi> \<xi>0) *\<^sub>V rep_c \<alpha>)\<close> for \<xi> :: 'a and \<alpha> :: \<open>'c\<close>
+  obtain f where bij_f: \<open>bij_betw f (UNIV::('a,'b) complement_domain set) (B \<xi>0)\<close>
+    apply atomize_elim apply (rule finite_same_card_bij)
+    using finiteB CARD_complement_domain[OF CARD'b] by auto
 
-  have cinner_u: \<open>cinner (u \<xi>\<alpha>) (u \<xi>'\<alpha>') = of_bool (\<xi>\<alpha> = \<xi>'\<alpha>')\<close> for \<xi>\<alpha> \<xi>'\<alpha>'
+  define u where \<open>u = (\<lambda>(\<xi>,\<alpha>). \<Phi> (butterket \<xi> \<xi>0) *\<^sub>V f \<alpha>)\<close> for \<xi> :: 'a and \<alpha> :: \<open>('a,'b) complement_domain\<close>
+  obtain U where Uapply: \<open>U *\<^sub>V ket \<xi>\<alpha> = u \<xi>\<alpha>\<close> for \<xi>\<alpha>
+    apply atomize_elim
+    apply (rule exI[of _ \<open>cblinfun_extension (range ket) (\<lambda>k. u (inv ket k))\<close>])
+    apply (subst cblinfun_extension_apply)
+      apply (rule cblinfun_extension_exists_finite_dim)
+    by (auto simp add: inj_ket cindependent_ket)
+
+  define eqa where \<open>eqa a b = (if a = b then 1 else 0 :: complex)\<close> for a b :: 'a
+  define eqc where \<open>eqc a b = (if a = b then 1 else 0 :: complex)\<close> for a b :: \<open>('a,'b) complement_domain\<close>
+  define eqac where \<open>eqac a b = (if a = b then 1 else 0 :: complex)\<close> for a b :: \<open>'a * ('a,'b) complement_domain\<close>
+
+  have \<open>cinner (U *\<^sub>V ket \<xi>\<alpha>) (U *\<^sub>V ket \<xi>'\<alpha>') = eqac \<xi>\<alpha> \<xi>'\<alpha>'\<close> for \<xi>\<alpha> \<xi>'\<alpha>'
   proof -
     obtain \<xi> \<alpha> \<xi>' \<alpha>' where \<xi>\<alpha>: \<open>\<xi>\<alpha> = (\<xi>,\<alpha>)\<close> and \<xi>'\<alpha>': \<open>\<xi>'\<alpha>' = (\<xi>',\<alpha>')\<close>
       apply atomize_elim by auto
-    have \<open>cinner (u (\<xi>,\<alpha>)) (u (\<xi>', \<alpha>')) = cinner (\<Phi> (butterket \<xi> \<xi>0) *\<^sub>V rep_c \<alpha>) (\<Phi> (butterket \<xi>' \<xi>0) *\<^sub>V rep_c \<alpha>')\<close>
-      unfolding u_def by simp
-    also have \<open>\<dots> = cinner ((\<Phi> (butterket \<xi>' \<xi>0))* *\<^sub>V \<Phi> (butterket \<xi> \<xi>0) *\<^sub>V rep_c \<alpha>) (rep_c \<alpha>')\<close>
+    have \<open>cinner (U *\<^sub>V ket (\<xi>,\<alpha>)) (U *\<^sub>V ket (\<xi>', \<alpha>')) = cinner (\<Phi> (butterket \<xi> \<xi>0) *\<^sub>V f \<alpha>) (\<Phi> (butterket \<xi>' \<xi>0) *\<^sub>V f \<alpha>')\<close>
+      unfolding Uapply u_def by simp
+    also have \<open>\<dots> = cinner ((\<Phi> (butterket \<xi>' \<xi>0))* *\<^sub>V \<Phi> (butterket \<xi> \<xi>0) *\<^sub>V f \<alpha>) (f \<alpha>')\<close>
       by (simp add: cinner_adj_left)
-    also have \<open>\<dots> = cinner (\<Phi> (butterket \<xi>' \<xi>0 *) *\<^sub>V \<Phi> (butterket \<xi> \<xi>0) *\<^sub>V rep_c \<alpha>) (rep_c \<alpha>')\<close>
+    also have \<open>\<dots> = cinner (\<Phi> (butterket \<xi>' \<xi>0 *) *\<^sub>V \<Phi> (butterket \<xi> \<xi>0) *\<^sub>V f \<alpha>) (f \<alpha>')\<close>
       by (metis (no_types, lifting) assms register_def)
-    also have \<open>\<dots> = cinner (\<Phi> (butterket \<xi>0 \<xi>' o\<^sub>C\<^sub>L butterket \<xi> \<xi>0) *\<^sub>V rep_c \<alpha>) (rep_c \<alpha>')\<close>
+    also have \<open>\<dots> = cinner (\<Phi> (butterket \<xi>0 \<xi>' o\<^sub>C\<^sub>L butterket \<xi> \<xi>0) *\<^sub>V f \<alpha>) (f \<alpha>')\<close>
       by (simp add: register_mult cblinfun_apply_cblinfun_compose[symmetric])
-    also have \<open>\<dots> = cinner (\<Phi> (of_bool (\<xi>'=\<xi>) *\<^sub>C selfbutterket \<xi>0) *\<^sub>V rep_c \<alpha>) (rep_c \<alpha>')\<close>
-      by (simp add: cinner_ket_left ket.rep_eq)
-    also have \<open>\<dots> = of_bool (\<xi>'=\<xi>) * cinner (\<Phi> (selfbutterket \<xi>0) *\<^sub>V rep_c \<alpha>) (rep_c \<alpha>')\<close>
-      by (simp add: complex_vector.linear_0)
-    also have \<open>\<dots> = of_bool (\<xi>'=\<xi>) * cinner (P' \<xi>0 *\<^sub>V rep_c \<alpha>) (rep_c \<alpha>')\<close>
-      using P_def P'_def by simp
-    also have \<open>\<dots> = of_bool (\<xi>'=\<xi>) * cinner (rep_c \<alpha>) (rep_c \<alpha>')\<close>
+    also have \<open>\<dots> = cinner (\<Phi> (eqa \<xi>' \<xi> *\<^sub>C selfbutterket \<xi>0) *\<^sub>V f \<alpha>) (f \<alpha>')\<close>
+      apply simp by (metis eqa_def cinner_ket)
+    also have \<open>\<dots> = eqa \<xi>' \<xi> * cinner (\<Phi> (selfbutterket \<xi>0) *\<^sub>V f \<alpha>) (f \<alpha>')\<close>
+      by (smt (verit, ccfv_threshold) \<open>clinear \<Phi>\<close> eqa_def cblinfun.scaleC_left cinner_commute 
+              cinner_scaleC_left cinner_zero_right complex_cnj_one complex_vector.linear_scale)
+    also have \<open>\<dots> = eqa \<xi>' \<xi> * cinner (P' \<xi>0 *\<^sub>V f \<alpha>) (f \<alpha>')\<close>
+      using P_butter P'_def by simp
+    also have \<open>\<dots> = eqa \<xi>' \<xi> * cinner (f \<alpha>) (f \<alpha>')\<close>
       apply (subst P'id)
-      apply (metis B\<xi>0 Rep ccspan_superset cspanB in_mono)
+       apply (metis bij_betw_imp_surj_on bij_f complex_vector.span_base cspanB rangeI)
       by simp
-    also have \<open>\<dots> = of_bool (\<xi>'=\<xi>) * of_bool (\<alpha>=\<alpha>')\<close>
-      using bij_rep_c orthoB normalB unfolding is_ortho_set_def
-      by (smt (verit, best) B\<xi>0 Rep Rep_inject cnorm_eq_1 of_bool_eq(1) of_bool_eq(2))
+    also have \<open>\<dots> = eqa \<xi>' \<xi> * eqc \<alpha> \<alpha>'\<close>
+      using bij_f orthoB normalB unfolding is_ortho_set_def eqc_def apply auto
+       apply (metis bij_betw_imp_surj_on cnorm_eq_1 rangeI)
+      by (smt (z3) bij_betw_iff_bijections iso_tuple_UNIV_I)
     finally show ?thesis
-      by (simp add: \<xi>'\<alpha>' \<xi>\<alpha>)
+      by (simp add: eqa_def eqac_def eqc_def \<xi>'\<alpha>' \<xi>\<alpha>)
   qed
-  define U where \<open>U = cblinfun_extension (range ket) (u o inv ket)\<close>
-  have Uapply: \<open>U *\<^sub>V ket \<xi>\<alpha> = u \<xi>\<alpha>\<close> for \<xi>\<alpha>
-    unfolding U_def
-    apply (subst cblinfun_extension_apply)
-    using cinner_u apply (auto intro!: cblinfun_extension_exists_ortho[where B=1])
-    by (metis (full_types) cinner_u cnorm_eq_1 of_bool_eq_1_iff order_refl)
-  have \<open>isometry U\<close>
+  then have \<open>isometry U\<close>
     apply (rule_tac orthogonal_on_basis_is_isometry[where B=\<open>range ket\<close>])
-    by (auto simp: Uapply cinner_u)
-  
-  have 1: \<open>U* o\<^sub>C\<^sub>L \<Phi> \<theta> o\<^sub>C\<^sub>L U = \<theta> \<otimes>\<^sub>o id_cblinfun\<close> for \<theta>
-  proof -
-    have *: \<open>U* o\<^sub>C\<^sub>L \<Phi> (butterket \<xi> \<eta>) o\<^sub>C\<^sub>L U = butterket \<xi> \<eta> \<otimes>\<^sub>o id_cblinfun\<close> for \<xi> \<eta>
-    proof (rule equal_ket, rename_tac \<xi>1\<alpha>)
-      fix \<xi>1\<alpha> obtain \<xi>1 :: 'a and \<alpha> :: \<open>'c\<close> where \<xi>1\<alpha>: \<open>\<xi>1\<alpha> = (\<xi>1,\<alpha>)\<close> 
-        apply atomize_elim by auto
-      have \<open>(U* o\<^sub>C\<^sub>L \<Phi> (butterket \<xi> \<eta>) o\<^sub>C\<^sub>L U) *\<^sub>V ket \<xi>1\<alpha> = U* *\<^sub>V \<Phi> (butterket \<xi> \<eta>) *\<^sub>V \<Phi> (butterket \<xi>1 \<xi>0) *\<^sub>V rep_c \<alpha>\<close>
-        unfolding cblinfun_apply_cblinfun_compose \<xi>1\<alpha> Uapply u_def by simp
-      also have \<open>\<dots> = U* *\<^sub>V \<Phi> (butterket \<xi> \<eta> o\<^sub>C\<^sub>L butterket \<xi>1 \<xi>0) *\<^sub>V rep_c \<alpha>\<close>
-        by (metis (no_types, lifting) assms butterfly_comp_butterfly lift_cblinfun_comp(4) register_mult)
-      also have \<open>\<dots> = U* *\<^sub>V \<Phi> (of_bool (\<eta>=\<xi>1) *\<^sub>C butterket \<xi> \<xi>0) *\<^sub>V rep_c \<alpha>\<close>
-        by (simp add: cinner_ket)
-      also have \<open>\<dots> = of_bool (\<eta>=\<xi>1) *\<^sub>C U* *\<^sub>V \<Phi> (butterket \<xi> \<xi>0) *\<^sub>V rep_c \<alpha>\<close>
-        by (simp add: complex_vector.linear_scale)
-      also have \<open>\<dots> = of_bool (\<eta>=\<xi>1) *\<^sub>C U* *\<^sub>V U *\<^sub>V ket (\<xi>, \<alpha>)\<close>
-        unfolding Uapply u_def by simp
-      also from \<open>isometry U\<close> have \<open>\<dots> = of_bool (\<eta>=\<xi>1) *\<^sub>C ket (\<xi>, \<alpha>)\<close>
-        unfolding cblinfun_apply_cblinfun_compose[symmetric] by simp
-      also have \<open>\<dots> = (butterket \<xi> \<eta> *\<^sub>V ket \<xi>1) \<otimes>\<^sub>s ket \<alpha>\<close>
-        by (simp add: tensor_ell2_scaleC1 tensor_ell2_ket)
-      also have \<open>\<dots> = (butterket \<xi> \<eta> \<otimes>\<^sub>o id_cblinfun) *\<^sub>V ket \<xi>1\<alpha>\<close>
-        by (simp add: \<xi>1\<alpha> tensor_op_ket)
-      finally show \<open>(U* o\<^sub>C\<^sub>L \<Phi> (butterket \<xi> \<eta>) o\<^sub>C\<^sub>L U) *\<^sub>V ket \<xi>1\<alpha> = (butterket \<xi> \<eta> \<otimes>\<^sub>o id_cblinfun) *\<^sub>V ket \<xi>1\<alpha>\<close>
-        by -
-    qed
+    using eqac_def by auto
 
-    have cont1: \<open>continuous_map weak_star_topology weak_star_topology (\<lambda>a. U* o\<^sub>C\<^sub>L \<Phi> a o\<^sub>C\<^sub>L U)\<close>
-      apply (subst asm_rl[of \<open>(\<lambda>a. U* o\<^sub>C\<^sub>L \<Phi> a o\<^sub>C\<^sub>L U) = (\<lambda>x. x o\<^sub>C\<^sub>L U) o (\<lambda>x. U* o\<^sub>C\<^sub>L x) o \<Phi>\<close>])
-      apply (auto intro!: continuous_map_compose[where X'=weak_star_topology])
-      using assms register_def continuous_map_left_comp_weak_star continuous_map_right_comp_weak_star by blast+
-
-    have *: \<open>U* o\<^sub>C\<^sub>L \<Phi> \<theta> o\<^sub>C\<^sub>L U = \<theta> \<otimes>\<^sub>o id_cblinfun\<close> if \<open>\<theta> \<in> cspan {butterket \<xi> \<eta> | \<xi> \<eta>. True}\<close> for \<theta>
-      apply (rule complex_vector.linear_eq_on[where x=\<theta>, OF _ _ that])
-        apply (intro \<open>clinear \<Phi>\<close>
-          clinear_compose[OF _ clinear_cblinfun_compose_left, unfolded o_def]
-          clinear_compose[OF _ clinear_cblinfun_compose_right, unfolded o_def])
-       apply simp
-      using * by blast
-    have \<open>U* o\<^sub>C\<^sub>L \<Phi> \<theta> o\<^sub>C\<^sub>L U = \<theta> \<otimes>\<^sub>o id_cblinfun\<close> 
-      if \<open>\<theta> \<in> (weak_star_topology closure_of (cspan {butterket \<xi> \<eta> | \<xi> \<eta>. True}))\<close> for \<theta>
-      apply (rule closure_of_eqI[OF _ _ that])
-      using * cont1 amplification_weak_star_cont by auto
-    with butterkets_weak_star_dense show ?thesis
-      by auto
+  have \<open>U* o\<^sub>C\<^sub>L \<Phi> (butterket \<xi> \<eta>) o\<^sub>C\<^sub>L U = butterket \<xi> \<eta> \<otimes>\<^sub>o id_cblinfun\<close> for \<xi> \<eta>
+  proof (rule equal_ket, rename_tac \<xi>1\<alpha>)
+    fix \<xi>1\<alpha> obtain \<xi>1 :: 'a and \<alpha> :: \<open>('a,'b) complement_domain\<close> where \<xi>1\<alpha>: \<open>\<xi>1\<alpha> = (\<xi>1,\<alpha>)\<close> 
+      apply atomize_elim by auto
+    have \<open>(U* o\<^sub>C\<^sub>L \<Phi> (butterket \<xi> \<eta>) o\<^sub>C\<^sub>L U) *\<^sub>V ket \<xi>1\<alpha> = U* *\<^sub>V \<Phi> (butterket \<xi> \<eta>) *\<^sub>V \<Phi> (butterket \<xi>1 \<xi>0) *\<^sub>V f \<alpha>\<close>
+      unfolding cblinfun_apply_cblinfun_compose \<xi>1\<alpha> Uapply u_def by simp
+    also have \<open>\<dots> = U* *\<^sub>V \<Phi> (butterket \<xi> \<eta> o\<^sub>C\<^sub>L butterket \<xi>1 \<xi>0) *\<^sub>V f \<alpha>\<close>
+      by (metis (no_types, lifting) assms butterfly_comp_butterfly lift_cblinfun_comp(4) register_mult)
+    also have \<open>\<dots> = U* *\<^sub>V \<Phi> (eqa \<eta> \<xi>1 *\<^sub>C butterket \<xi> \<xi>0) *\<^sub>V f \<alpha>\<close>
+      by (simp add: eqa_def cinner_ket)
+    also have \<open>\<dots> = eqa \<eta> \<xi>1 *\<^sub>C U* *\<^sub>V \<Phi> (butterket \<xi> \<xi>0) *\<^sub>V f \<alpha>\<close>
+      by (simp add: complex_vector.linear_scale)
+    also have \<open>\<dots> = eqa \<eta> \<xi>1 *\<^sub>C U* *\<^sub>V U *\<^sub>V ket (\<xi>, \<alpha>)\<close>
+      unfolding Uapply u_def by simp
+    also from \<open>isometry U\<close> have \<open>\<dots> = eqa \<eta> \<xi>1 *\<^sub>C ket (\<xi>, \<alpha>)\<close>
+      unfolding cblinfun_apply_cblinfun_compose[symmetric] by simp
+    also have \<open>\<dots> = (butterket \<xi> \<eta> *\<^sub>V ket \<xi>1) \<otimes>\<^sub>s ket \<alpha>\<close>
+      by (simp add: eqa_def tensor_ell2_scaleC1)
+    also have \<open>\<dots> = (butterket \<xi> \<eta> \<otimes>\<^sub>o id_cblinfun) *\<^sub>V ket \<xi>1\<alpha>\<close>
+      by (simp add: \<xi>1\<alpha> tensor_op_ket)
+    finally show \<open>(U* o\<^sub>C\<^sub>L \<Phi> (butterket \<xi> \<eta>) o\<^sub>C\<^sub>L U) *\<^sub>V ket \<xi>1\<alpha> = (butterket \<xi> \<eta> \<otimes>\<^sub>o id_cblinfun) *\<^sub>V ket \<xi>1\<alpha>\<close>
+      by -
   qed
+  then have 1: \<open>U* o\<^sub>C\<^sub>L \<Phi> \<theta> o\<^sub>C\<^sub>L U = \<theta> \<otimes>\<^sub>o id_cblinfun\<close> for \<theta>
+    apply (rule_tac clinear_eq_butterfly_ketI[THEN fun_cong, where x=\<theta>])
+    by (auto intro!: clinearI simp add: bounded_cbilinear.add_left bounded_cbilinear_cblinfun_compose complex_vector.linear_add complex_vector.linear_scale)
+
   have \<open>unitary U\<close>
   proof -
     have \<open>\<Phi> (butterket \<xi> \<xi>1) *\<^sub>S \<top> \<le> U *\<^sub>S \<top>\<close> for \<xi> \<xi>1
     proof -
       have *: \<open>\<Phi> (butterket \<xi> \<xi>0) *\<^sub>V b \<in> space_as_set (U *\<^sub>S \<top>)\<close> if \<open>b \<in> B \<xi>0\<close> for b
-        apply (subst asm_rl[of \<open>\<Phi> (butterket \<xi> \<xi>0) *\<^sub>V b = u (\<xi>, inv rep_c b)\<close>])
-         apply (simp add: u_def, metis bij_betw_inv_into_right bij_rep_c that)
+        apply (subst asm_rl[of \<open>\<Phi> (butterket \<xi> \<xi>0) *\<^sub>V b = u (\<xi>, inv f b)\<close>])
+         apply (simp add: u_def, metis bij_betw_inv_into_right bij_f that)
         by (metis Uapply cblinfun_apply_in_image)
 
       have \<open>\<Phi> (butterket \<xi> \<xi>1) *\<^sub>S \<top> = \<Phi> (butterket \<xi> \<xi>0) *\<^sub>S \<Phi> (butterket \<xi>0 \<xi>0) *\<^sub>S \<Phi> (butterket \<xi>0 \<xi>1) *\<^sub>S \<top>\<close>
@@ -879,38 +288,24 @@ proof (rule with_typeI; unfold fst_conv snd_conv)
       also have \<open>\<dots> \<le> \<Phi> (butterket \<xi> \<xi>0) *\<^sub>S \<Phi> (butterket \<xi>0 \<xi>0) *\<^sub>S \<top>\<close>
         by (meson cblinfun_image_mono top_greatest)
       also have \<open>\<dots> = \<Phi> (butterket \<xi> \<xi>0) *\<^sub>S S \<xi>0\<close>
-        by (simp add: S_def P'_def P_def)
+        by (simp add: S_def P'_def P_butter)
       also have \<open>\<dots> = \<Phi> (butterket \<xi> \<xi>0) *\<^sub>S ccspan (B \<xi>0)\<close>
-        by (simp add: cspanB)
+        by (simp add: ccspanB)
       also have \<open>\<dots> = ccspan (\<Phi> (butterket \<xi> \<xi>0) ` B \<xi>0)\<close>
         by (meson cblinfun_image_ccspan)
       also have \<open>\<dots> \<le> U *\<^sub>S \<top>\<close>
         by (rule ccspan_leqI, use * in auto)
       finally show ?thesis by -
     qed
-    then have \<open>ccspan {\<Phi> (butterket \<xi> \<xi>) *\<^sub>V \<alpha> |\<xi> \<alpha>. True} \<le> U *\<^sub>S \<top>\<close>
-      apply (rule_tac ccspan_leqI)
-      using cblinfun_apply_in_image less_eq_ccsubspace.rep_eq by blast
-    moreover have \<open>ccspan {\<Phi> (butterket \<xi> \<xi>) *\<^sub>V \<alpha> |\<xi> \<alpha>. True} = \<top>\<close>
-    proof -
-      define Q where \<open>Q = Proj (- ccspan {\<Phi> (butterket \<xi> \<xi>) *\<^sub>V \<alpha> |\<xi> \<alpha>. True})\<close>
-      have \<open>has_sum_in weak_star_topology (\<lambda>\<xi>. Q o\<^sub>C\<^sub>L \<Phi> (butterket \<xi> \<xi>)) UNIV (Q o\<^sub>C\<^sub>L id_cblinfun)\<close>
-        apply (rule has_sum_in_comm_additive[where g=\<open>cblinfun_compose Q\<close> and T=weak_star_topology, unfolded o_def])
-        using sumP'id2
-        by (auto simp add: continuous_map_left_comp_weak_star P'_def P_def cblinfun_compose_add_right)
-      moreover have \<open>Q o\<^sub>C\<^sub>L \<Phi> (butterket \<xi> \<xi>) = 0\<close> for \<xi>
-        apply (auto intro!: equal_ket simp: Q_def Proj_ortho_compl cblinfun.diff_left)
-        apply (subst Proj_fixes_image)
-        by (auto intro!: ccspan_superset[THEN set_mp])
-      ultimately have \<open>Q = 0\<close>
-        apply (rule_tac has_sum_in_unique)
-        by auto
-      then show ?thesis
-        apply (auto simp: Q_def)
-        by (smt (verit, del_insts) Proj_ortho_compl Proj_range cblinfun_image_id right_minus_eq)
-    qed
-    ultimately have \<open>U *\<^sub>S \<top> = \<top>\<close>
-      by (simp add: top.extremum_unique)
+    moreover have \<open>\<Phi> id_cblinfun *\<^sub>S \<top> \<le> (SUP \<xi>\<in>UNIV. \<Phi> (selfbutterket \<xi>) *\<^sub>S \<top>)\<close>
+      unfolding sum_butterfly_ket[symmetric]
+      apply (subst complex_vector.linear_sum, simp)
+      by (rule cblinfun_sum_image_distr)
+    ultimately have \<open>\<Phi> id_cblinfun *\<^sub>S \<top> \<le> U *\<^sub>S \<top>\<close>
+      apply auto by (meson SUP_le_iff order.trans)
+    then have \<open>U *\<^sub>S \<top> = \<top>\<close>
+      apply auto
+      using top.extremum_unique by blast
     with \<open>isometry U\<close> show \<open>unitary U\<close>
       by (rule surj_isometry_is_unitary)
   qed
@@ -928,7 +323,7 @@ proof (rule with_typeI; unfold fst_conv snd_conv)
       by -
   qed
 
-  with \<open>unitary U\<close> show \<open>\<exists>U :: ('a \<times> 'c) ell2 \<Rightarrow>\<^sub>C\<^sub>L 'b ell2. unitary U \<and> (\<forall>\<theta>. \<Phi> \<theta> = Misc.sandwich U (\<theta> \<otimes>\<^sub>o id_cblinfun))\<close>
+  with \<open>unitary U\<close> show ?thesis
     by (auto simp: sandwich_def)
 qed
 
@@ -938,179 +333,133 @@ lemma register_decomposition_converse:
   using _ unitary_sandwich_register apply (rule register_comp[unfolded o_def])
   using assms by auto
 
-lemma register_inj: \<open>inj F\<close> if [simp]: \<open>register F\<close>
+
+lemma register_inj: \<open>inj F\<close> if \<open>register F\<close>
 proof -
-  have \<open>\<forall>\<^sub>\<tau> 'c::type = register_decomposition_basis F. inj F\<close>
-    using register_decomposition[OF \<open>register F\<close>] 
-  proof (rule with_type_mp)
-    fix rep :: \<open>'c \<Rightarrow> 'd\<close> and abs and S
-    assume \<open>type_definition rep abs S\<close>
-    assume \<open>\<exists>U :: ('a \<times> 'c) ell2 \<Rightarrow>\<^sub>C\<^sub>L 'b ell2. unitary U \<and> (\<forall>\<theta>. F \<theta> = sandwich U (\<theta> \<otimes>\<^sub>o id_cblinfun))\<close>
-    then obtain U :: \<open>('a \<times> 'c) ell2 \<Rightarrow>\<^sub>C\<^sub>L 'b ell2\<close>
-      where \<open>unitary U\<close> and F: \<open>F a = sandwich U (a \<otimes>\<^sub>o id_cblinfun)\<close> for a
-      apply atomize_elim by auto
-    have \<open>inj (sandwich U)\<close>
-      by (smt (verit, best) \<open>unitary U\<close> cblinfun_assoc_left inj_onI sandwich_def cblinfun_compose_id_right cblinfun_compose_id_left unitary_def)
-    moreover have \<open>inj (\<lambda>a::'a ell2 \<Rightarrow>\<^sub>C\<^sub>L _. a \<otimes>\<^sub>o id_cblinfun)\<close>
-      by (rule inj_tensor_left, simp)
-    ultimately show \<open>inj F\<close>
-      unfolding F
-      by (smt (z3) inj_def)
-  qed
-  from this[THEN with_type_prepare_cancel, cancel_type_definition, OF with_type_nonempty, OF this]
-  show \<open>inj F\<close>
-    by -
+  obtain U :: \<open>('a \<times> ('a, 'b) complement_domain) ell2 \<Rightarrow>\<^sub>C\<^sub>L 'b ell2\<close>
+    where \<open>unitary U\<close> and F: \<open>F a = sandwich U (a \<otimes>\<^sub>o id_cblinfun)\<close> for a
+    apply atomize_elim using \<open>register F\<close> by (rule register_decomposition)
+  have \<open>inj (sandwich U)\<close>
+    by (smt (verit, best) \<open>unitary U\<close> cblinfun_assoc_left inj_onI sandwich_def cblinfun_compose_id_right cblinfun_compose_id_left unitary_def)
+  moreover have \<open>inj (\<lambda>a::'a::finite ell2 \<Rightarrow>\<^sub>C\<^sub>L _. a \<otimes>\<^sub>o id_cblinfun)\<close>
+    by (rule inj_tensor_left, simp)
+  ultimately show \<open>inj F\<close>
+    unfolding F
+    by (smt (z3) inj_def) 
 qed
-
-
-lemma weak_star_clinear_eq_butterfly_ketI:
-  fixes F G :: \<open>('a ell2 \<Rightarrow>\<^sub>C\<^sub>L 'b ell2) \<Rightarrow> 'c::complex_vector\<close>
-  assumes "clinear F" and "clinear G"
-    and \<open>continuous_map weak_star_topology T F\<close> and \<open>continuous_map weak_star_topology T G\<close>
-    and \<open>hausdorff T\<close>
-  assumes "\<And>i j. F (butterfly (ket i) (ket j)) = G (butterfly (ket i) (ket j))"
-  shows "F = G"
-proof -
-  have FG: \<open>F x = G x\<close> if \<open>x \<in> cspan {butterket i j |i j. True}\<close> for x
-    by (smt (verit, ccfv_threshold) assms(1) assms(2) assms(6) complex_vector.linear_eq_on mem_Collect_eq that)
-  show ?thesis
-    apply (rule ext)
-    using \<open>hausdorff T\<close> FG
-    apply (rule closure_of_eqI[where f=F and g=G and S=\<open>cspan {butterket i j| i j. True}\<close>])
-    using assms butterkets_weak_star_dense by auto
-qed
-
-lemma clinear_register: \<open>register F \<Longrightarrow> clinear F\<close>
-  using bounded_clinear.clinear register_bounded_clinear by blast
-
-lemma weak_star_cont_register: \<open>register F \<Longrightarrow> continuous_map weak_star_topology weak_star_topology F\<close>
-  using register_def by blast
 
 lemma iso_register_decomposition:
   assumes [simp]: \<open>iso_register F\<close>
   shows \<open>\<exists>U. unitary U \<and> F = sandwich U\<close>
 proof -
-  from register_decomposition
-  have \<open>\<forall>\<^sub>\<tau> 'c::type = register_decomposition_basis F.
-        \<exists>U. unitary U \<and> F = sandwich U\<close>
-  proof (rule with_type_mp)
-    show [simp]: \<open>register F\<close>
-      using assms iso_register_is_register by blast 
+  have [simp]: \<open>register F\<close>
+    using assms iso_register_is_register by blast 
 
-    assume register_decomposition:
-      \<open>\<exists>U :: ('a \<times> 'c) ell2 \<Rightarrow>\<^sub>C\<^sub>L 'b ell2. unitary U \<and> (\<forall>\<theta>. F \<theta> = Misc.sandwich U (\<theta> \<otimes>\<^sub>o id_cblinfun))\<close>
+  let ?ida = \<open>id_cblinfun :: ('a, 'b) complement_domain ell2 \<Rightarrow>\<^sub>C\<^sub>L _\<close>
 
-    let ?ida = \<open>id_cblinfun :: 'c ell2 \<Rightarrow>\<^sub>C\<^sub>L _\<close>
+  from register_decomposition[OF \<open>register F\<close>]
+  obtain V :: \<open>('a \<times> ('a, 'b) complement_domain) ell2 \<Rightarrow>\<^sub>C\<^sub>L 'b ell2\<close> where \<open>unitary V\<close>
+    and FV: \<open>F \<theta> = sandwich V (\<theta> \<otimes>\<^sub>o ?ida)\<close> for \<theta>
+    by auto
 
-    from register_decomposition
-    obtain V :: \<open>('a \<times> 'c) ell2 \<Rightarrow>\<^sub>C\<^sub>L 'b ell2\<close> where \<open>unitary V\<close>
-      and FV: \<open>F \<theta> = sandwich V (\<theta> \<otimes>\<^sub>o ?ida)\<close> for \<theta>
-      by auto
+  have \<open>surj F\<close>
+    by (meson assms iso_register_inv_comp2 surj_iff)
+  have surj_tensor: \<open>surj (\<lambda>a::'a ell2 \<Rightarrow>\<^sub>C\<^sub>L 'a ell2. a \<otimes>\<^sub>o ?ida)\<close>
+    apply (rule surj_from_comp[where g=\<open>sandwich V\<close>])
+    using \<open>surj F\<close> apply (auto simp: FV)
+    by (meson \<open>unitary V\<close> register_inj unitary_sandwich_register)
+  then obtain a :: \<open>'a ell2 \<Rightarrow>\<^sub>C\<^sub>L _\<close> 
+    where a: \<open>a \<otimes>\<^sub>o ?ida = selfbutterket undefined \<otimes>\<^sub>o selfbutterket undefined\<close>
+    by (smt (verit, best) surjD)
 
-    have \<open>surj F\<close>
-      by (meson assms iso_register_inv_comp2 surj_iff)
-    have surj_tensor: \<open>surj (\<lambda>a::'a ell2 \<Rightarrow>\<^sub>C\<^sub>L 'a ell2. a \<otimes>\<^sub>o ?ida)\<close>
-      apply (rule surj_from_comp[where g=\<open>sandwich V\<close>])
-      using \<open>surj F\<close> apply (auto simp: FV)
-      by (meson \<open>unitary V\<close> register_inj unitary_sandwich_register)
-    then obtain a :: \<open>'a ell2 \<Rightarrow>\<^sub>C\<^sub>L _\<close> 
-      where a: \<open>a \<otimes>\<^sub>o ?ida = selfbutterket undefined \<otimes>\<^sub>o selfbutterket undefined\<close>
-      by (smt (verit, best) surjD)
+  then have \<open>a \<noteq> 0\<close>
+    apply auto
+    by (metis butterfly_apply cblinfun.zero_left complex_vector.scale_eq_0_iff ket_nonzero orthogonal_ket)
 
-    then have \<open>a \<noteq> 0\<close>
-      apply (auto simp: tensor_ell2_ket)
-      by (metis butterfly_apply cblinfun.zero_left complex_vector.scale_eq_0_iff ket_nonzero orthogonal_ket)
+  obtain \<gamma> where \<gamma>: \<open>?ida = \<gamma> *\<^sub>C selfbutterket undefined\<close>
+    apply atomize_elim
+    using a \<open>a \<noteq> 0\<close> by (rule tensor_op_almost_injective)
+  then have \<open>?ida (ket undefined) = \<gamma> *\<^sub>C (selfbutterket undefined *\<^sub>V ket undefined)\<close>
+    by (simp add: \<open>id_cblinfun = \<gamma> *\<^sub>C selfbutterket undefined\<close> scaleC_cblinfun.rep_eq)
+  then have \<open>ket undefined = \<gamma> *\<^sub>C ket undefined\<close>
+    by (metis butterfly_apply cinner_scaleC_right id_cblinfun_apply cinner_ket_same mult.right_neutral scaleC_one)
+  then have \<open>\<gamma> = 1\<close>
+    by (smt (z3) \<gamma> butterfly_apply butterfly_scaleC_left cblinfun_id_cblinfun_apply complex_vector.scale_cancel_right cinner_ket_same ket_nonzero)
 
-    obtain \<gamma> where \<gamma>: \<open>?ida = \<gamma> *\<^sub>C selfbutterket undefined\<close>
-      apply atomize_elim
-      using a \<open>a \<noteq> 0\<close> by (rule tensor_op_almost_injective)
-    then have \<open>?ida (ket undefined) = \<gamma> *\<^sub>C (selfbutterket undefined *\<^sub>V ket undefined)\<close>
-      by (simp add: \<open>id_cblinfun = \<gamma> *\<^sub>C selfbutterket undefined\<close> scaleC_cblinfun.rep_eq)
-    then have \<open>ket undefined = \<gamma> *\<^sub>C ket undefined\<close>
-      by (metis butterfly_apply cinner_ket_same id_cblinfun_apply ket_nonzero scaleC_cancel_right scaleC_one)
-    then have \<open>\<gamma> = 1\<close>
-      by (smt (z3) \<gamma> butterfly_apply butterfly_scaleC_left cblinfun_id_cblinfun_apply complex_vector.scale_cancel_right cinner_ket_same ket_nonzero)
+  define T U where \<open>T = CBlinfun (\<lambda>\<psi>. \<psi> \<otimes>\<^sub>s ket undefined)\<close> and \<open>U = V o\<^sub>C\<^sub>L T\<close>
+  have T: \<open>T \<psi> = \<psi> \<otimes>\<^sub>s ket undefined\<close> for \<psi>
+    unfolding T_def
+    apply (subst bounded_clinear_CBlinfun_apply)
+    by (auto intro!: bounded_clinear_finite_dim clinear_tensor_ell22)
+  have sandwich_T: \<open>sandwich T a = a \<otimes>\<^sub>o ?ida\<close> for a
+    apply (rule fun_cong[where x=a])
+    apply (rule clinear_eq_butterfly_ketI)
+      apply auto
+    by (metis (no_types, opaque_lifting) Misc.sandwich_def T \<gamma> \<open>\<gamma> = 1\<close> adj_cblinfun_compose butterfly_adjoint cblinfun_comp_butterfly scaleC_one tensor_butterfly)
 
-    define T U where \<open>T = CBlinfun (\<lambda>\<psi>. \<psi> \<otimes>\<^sub>s ket undefined)\<close> and \<open>U = V o\<^sub>C\<^sub>L T\<close>
-    have T: \<open>T \<psi> = \<psi> \<otimes>\<^sub>s ket undefined\<close> for \<psi>
-      unfolding T_def
-      apply (subst bounded_clinear_CBlinfun_apply)
-      by (auto intro!: bounded_clinear_tensor_ell22)
-    have \<open>sandwich T (butterket i j) = butterket i j \<otimes>\<^sub>o id_cblinfun\<close> for i j
-      by (simp add: T sandwich_def cblinfun_comp_butterfly butterfly_comp_cblinfun \<gamma> \<open>\<gamma> = 1\<close>)
-    then have sandwich_T: \<open>sandwich T a = a \<otimes>\<^sub>o ?ida\<close> for a
-      apply (rule_tac fun_cong[where x=a])
-      apply (rule weak_star_clinear_eq_butterfly_ketI[where T=weak_star_topology])
-      by auto
+  have \<open>F (butterfly x y) = V o\<^sub>C\<^sub>L (butterfly x y \<otimes>\<^sub>o ?ida) o\<^sub>C\<^sub>L V*\<close> for x y
+    by (simp add: Misc.sandwich_def FV)
+  also have \<open>\<dots> x y = V o\<^sub>C\<^sub>L (butterfly (T x) (T y)) o\<^sub>C\<^sub>L V*\<close> for x y
+    by (simp add: T \<gamma> \<open>\<gamma> = 1\<close>)
+  also have \<open>\<dots> x y = U o\<^sub>C\<^sub>L (butterfly x y) o\<^sub>C\<^sub>L U*\<close> for x y
+    by (simp add: U_def butterfly_comp_cblinfun cblinfun_comp_butterfly)
+  finally have F_rep:  \<open>F a = U o\<^sub>C\<^sub>L a o\<^sub>C\<^sub>L U*\<close> for a
+    apply (rule_tac fun_cong[where x=a])
+    apply (rule_tac clinear_eq_butterfly_ketI)
+      apply auto
+    by (metis (no_types, lifting) cblinfun_apply_clinear clinear_iff sandwich_apply)
 
-    have \<open>F (butterfly x y) = V o\<^sub>C\<^sub>L (butterfly x y \<otimes>\<^sub>o ?ida) o\<^sub>C\<^sub>L V*\<close> for x y
-      by (simp add: Misc.sandwich_def FV)
-    also have \<open>\<dots> x y = V o\<^sub>C\<^sub>L (butterfly (T x) (T y)) o\<^sub>C\<^sub>L V*\<close> for x y
-      by (simp add: T \<gamma> \<open>\<gamma> = 1\<close>)
-    also have \<open>\<dots> x y = U o\<^sub>C\<^sub>L (butterfly x y) o\<^sub>C\<^sub>L U*\<close> for x y
-      by (simp add: U_def butterfly_comp_cblinfun cblinfun_comp_butterfly)
-    finally have F_rep:  \<open>F a = U o\<^sub>C\<^sub>L a o\<^sub>C\<^sub>L U*\<close> for a
-      apply (rule_tac fun_cong[where x=a])
-      apply (rule weak_star_clinear_eq_butterfly_ketI[where T=weak_star_topology])
-      by (auto simp: clinear_register weak_star_cont_register simp flip: sandwich_def)
-
-    have \<open>isometry T\<close>
-      apply (rule orthogonal_on_basis_is_isometry[where B=\<open>range ket\<close>])
-      by (auto simp: T)
-    moreover have \<open>T *\<^sub>S \<top> = \<top>\<close>
+  have \<open>isometry T\<close>
+    apply (rule orthogonal_on_basis_is_isometry[where B=\<open>range ket\<close>])
+    by (auto simp: T)
+  moreover have \<open>T *\<^sub>S \<top> = \<top>\<close>
+  proof -
+    have 1: \<open>\<phi> \<otimes>\<^sub>s \<xi> \<in> range ((*\<^sub>V) T)\<close> for \<phi> \<xi>
     proof -
-      have 1: \<open>\<phi> \<otimes>\<^sub>s \<xi> \<in> range ((*\<^sub>V) T)\<close> for \<phi> \<xi>
-      proof -
-        have \<open>T *\<^sub>V (cinner (ket undefined) \<xi> *\<^sub>C \<phi>) = \<phi> \<otimes>\<^sub>s (cinner (ket undefined) \<xi> *\<^sub>C ket undefined)\<close>
-          by (simp add: T tensor_ell2_scaleC1 tensor_ell2_scaleC2)
-        also have \<open>\<dots> = \<phi> \<otimes>\<^sub>s (selfbutterket undefined *\<^sub>V \<xi>)\<close>
-          by simp
-        also have \<open>\<dots> = \<phi> \<otimes>\<^sub>s (?ida *\<^sub>V \<xi>)\<close>
-          by (simp add: \<gamma> \<open>\<gamma> = 1\<close>)
-        also have \<open>\<dots> = \<phi> \<otimes>\<^sub>s \<xi>\<close>
-          by simp
-        finally show ?thesis
-          by (metis range_eqI)
-      qed
-
-      have \<open>\<top> \<le> ccspan {ket x | x. True}\<close>
-        by (simp add: full_SetCompr_eq)
-      also have \<open>\<dots> \<le> ccspan {\<phi> \<otimes>\<^sub>s \<xi> | \<phi> \<xi>. True}\<close>
-        apply (rule ccspan_mono)
-        by (auto simp flip: tensor_ell2_ket)
-      also from 1 have \<open>\<dots> \<le> ccspan (range ((*\<^sub>V) T))\<close>
-        by (auto intro!: ccspan_mono)
-      also have \<open>\<dots> = T *\<^sub>S \<top>\<close>
-        by (metis (mono_tags, opaque_lifting) calculation cblinfun_image_ccspan cblinfun_image_mono eq_iff top_greatest)
-      finally show \<open>T *\<^sub>S \<top> = \<top>\<close>
-        using top.extremum_uniqueI by blast
+      have \<open>T *\<^sub>V (cinner (ket undefined) \<xi> *\<^sub>C \<phi>) = \<phi> \<otimes>\<^sub>s (cinner (ket undefined) \<xi> *\<^sub>C ket undefined)\<close>
+        by (simp add: T tensor_ell2_scaleC2)
+      also have \<open>\<dots> = \<phi> \<otimes>\<^sub>s (selfbutterket undefined *\<^sub>V \<xi>)\<close>
+        by simp
+      also have \<open>\<dots> = \<phi> \<otimes>\<^sub>s (?ida *\<^sub>V \<xi>)\<close>
+        by (simp add: \<gamma> \<open>\<gamma> = 1\<close>)
+      also have \<open>\<dots> = \<phi> \<otimes>\<^sub>s \<xi>\<close>
+        by simp
+      finally show ?thesis
+        by (metis range_eqI)
     qed
 
-    ultimately have \<open>unitary T\<close>
-      by (rule surj_isometry_is_unitary)
-    then have \<open>unitary U\<close>
-      by (simp add: U_def \<open>unitary V\<close>)
-
-    from F_rep \<open>unitary U\<close> show \<open>\<exists>U. unitary U \<and> F = Misc.sandwich U\<close>
-      by (auto simp: sandwich_def[abs_def])
+    have \<open>\<top> \<le> ccspan {ket x | x. True}\<close>
+      by (simp add: full_SetCompr_eq)
+    also have \<open>\<dots> \<le> ccspan {\<phi> \<otimes>\<^sub>s \<xi> | \<phi> \<xi>. True}\<close>
+      apply (rule ccspan_mono)
+      by (auto simp flip: tensor_ell2_ket)
+    also from 1 have \<open>\<dots> \<le> ccspan (range ((*\<^sub>V) T))\<close>
+      by (auto intro!: ccspan_mono)
+    also have \<open>\<dots> = T *\<^sub>S \<top>\<close>
+      by (metis (mono_tags, opaque_lifting) calculation cblinfun_image_ccspan cblinfun_image_mono eq_iff top_greatest)
+    finally show \<open>T *\<^sub>S \<top> = \<top>\<close>
+      using top.extremum_uniqueI by blast
   qed
-  from this[THEN with_type_prepare_cancel, cancel_type_definition, OF with_type_nonempty, OF this]
-  show ?thesis
-    by -
+
+  ultimately have \<open>unitary T\<close>
+    by (rule surj_isometry_is_unitary)
+  then have \<open>unitary U\<close>
+    by (simp add: U_def \<open>unitary V\<close>)
+
+  from F_rep \<open>unitary U\<close> show ?thesis
+    by (auto simp: sandwich_def[abs_def])
 qed
 
 lemma complement_exists:
-  fixes F :: \<open>'a update \<Rightarrow> 'b update\<close>
+  fixes F :: \<open>'a::finite update \<Rightarrow> 'b::finite update\<close>
   assumes \<open>register F\<close>
-  shows \<open>\<forall>\<^sub>\<tau> 'c::type = register_decomposition_basis F.
-         \<exists>G :: 'c update \<Rightarrow> 'b update. compatible F G \<and> iso_register (F;G)\<close>
-proof (use register_decomposition[OF \<open>register F\<close>] in \<open>rule with_type_mp\<close>)
+  shows \<open>\<exists>G :: ('a, 'b) complement_domain update \<Rightarrow> 'b update. compatible F G \<and> iso_register (F;G)\<close>
+proof -
   note [[simproc del: Laws_Quantum.compatibility_warn]]
-  assume register_decomposition: \<open>\<exists>U :: ('a \<times> 'c) ell2 \<Rightarrow>\<^sub>C\<^sub>L 'b ell2. unitary U \<and> (\<forall>\<theta>. F \<theta> = Misc.sandwich U (\<theta> \<otimes>\<^sub>o id_cblinfun))\<close>
-  then obtain U :: \<open>('a \<times> 'c) ell2 \<Rightarrow>\<^sub>C\<^sub>L 'b ell2\<close>
+  obtain U :: \<open>('a \<times> ('a, 'b) complement_domain) ell2 \<Rightarrow>\<^sub>C\<^sub>L 'b ell2\<close>
     where [simp]: "unitary U" and F: \<open>F a = sandwich U (a \<otimes>\<^sub>o id_cblinfun)\<close> for a
-    by auto
-  define G :: \<open>'c update \<Rightarrow> 'b update\<close> where \<open>G b = sandwich U (id_cblinfun \<otimes>\<^sub>o b)\<close> for b
+    apply atomize_elim using assms by (rule register_decomposition)
+  define G :: \<open>(('a, 'b) complement_domain) update \<Rightarrow> 'b update\<close> where \<open>G b = sandwich U (id_cblinfun \<otimes>\<^sub>o b)\<close> for b
   have [simp]: \<open>register G\<close>
     unfolding G_def apply (rule register_decomposition_converse) by simp
   have \<open>F a o\<^sub>C\<^sub>L G b = G b o\<^sub>C\<^sub>L F a\<close> for a b
@@ -1124,7 +473,7 @@ proof (use register_decomposition[OF \<open>register F\<close>] in \<open>rule w
     ultimately show ?thesis by simp
   qed
   then have [simp]: \<open>compatible F G\<close>
-    by (auto simp: compatible_def \<open>register F\<close>)
+    by (auto simp: compatible_def \<open>register F\<close> \<open>register G\<close>)
   moreover have \<open>iso_register (F;G)\<close>
   proof -
     have \<open>(F;G) (a \<otimes>\<^sub>o b) = sandwich U (a \<otimes>\<^sub>o b)\<close> for a b
@@ -1132,7 +481,7 @@ proof (use register_decomposition[OF \<open>register F\<close>] in \<open>rule w
       by (metis (no_types, lifting) \<open>unitary U\<close> isometryD cblinfun_assoc_left(1) comp_tensor_op cblinfun_compose_id_right cblinfun_compose_id_left unitary_isometry)
     then have FG: \<open>(F;G) = sandwich U\<close>
       apply (rule tensor_extensionality[rotated -1])
-      by (simp_all add: unitary_sandwich_register)
+      by (simp_all add: bounded_cbilinear.add_left bounded_cbilinear_cblinfun_compose bounded_cbilinear.add_right clinearI)
     define I where \<open>I = sandwich (U*)\<close> for x
     have [simp]: \<open>register I\<close>
       by (simp add: I_def unitary_sandwich_register)
@@ -1143,47 +492,14 @@ proof (use register_decomposition[OF \<open>register F\<close>] in \<open>rule w
     then show \<open>iso_register (F;G)\<close>
       by (auto intro!: iso_registerI)
   qed
-  ultimately show \<open>\<exists>G :: 'c update \<Rightarrow> 'b update. compatible F G \<and> iso_register (F;G)\<close>
-    apply (rule_tac exI[of _ G]) by auto
+  ultimately show ?thesis
+    apply (rule_tac exI[of _ G]) by (auto)
 qed
 
 definition \<open>commutant F = {x. \<forall>y\<in>F. x o\<^sub>C\<^sub>L y = y o\<^sub>C\<^sub>L x}\<close>
 
-(* TODO move *)
-lemma norm_isometry_o: \<open>norm (U o\<^sub>C\<^sub>L A) = norm A\<close> if \<open>isometry U\<close>
-  by (smt (verit, del_insts) cblinfun_compose_id_left compatible_ac_rules(2) isometryD isometry_partial_isometry mult_cancel_left2 mult_cancel_right1 norm_adj norm_cblinfun_compose norm_eq_zero norm_le_zero_iff norm_partial_isometry that)
-
-(* TODO move *)
-lemma norm_isometry_o': \<open>norm (A o\<^sub>C\<^sub>L U) = norm A\<close> if \<open>isometry (U*)\<close>
-  by (smt (verit, ccfv_threshold) adj_0 cblinfun_assoc_right(1) cblinfun_compose_id_right cblinfun_compose_zero_right double_adj isometryD isometry_partial_isometry mult_cancel_left2 norm_adj norm_cblinfun_compose norm_partial_isometry norm_zero that)
-
-lemma register_norm: \<open>norm (F a) = norm a\<close> if \<open>register F\<close>
-proof -
-  have \<open>\<forall>\<^sub>\<tau> 'c::type = register_decomposition_basis F.
-         (\<exists>U :: ('a \<times> 'c) ell2 \<Rightarrow>\<^sub>C\<^sub>L 'b ell2. unitary U \<and> 
-              (\<forall>\<theta>. F \<theta> = sandwich U (\<theta> \<otimes>\<^sub>o id_cblinfun)))\<close>
-    (* using complement_exists that by blast *)
-    using register_decomposition that by blast
-  then have \<open>\<forall>\<^sub>\<tau> 'c::type = register_decomposition_basis F.
-         norm (F a) = norm a\<close>
-  proof (rule with_type_mp) 
-    fix Rep :: \<open>'c \<Rightarrow> 'b ell2\<close> and Abs
-    assume \<open>type_definition Rep Abs (register_decomposition_basis F)\<close>
-    assume \<open>(\<exists>U :: ('a \<times> 'c) ell2 \<Rightarrow>\<^sub>C\<^sub>L 'b ell2. unitary U \<and> 
-              (\<forall>\<theta>. F \<theta> = sandwich U (\<theta> \<otimes>\<^sub>o id_cblinfun)))\<close>
-    then obtain U :: \<open>('a \<times> 'c) ell2 \<Rightarrow>\<^sub>C\<^sub>L 'b ell2\<close> where \<open>unitary U\<close>
-      and FU: \<open>F \<theta> = sandwich U (\<theta> \<otimes>\<^sub>o id_cblinfun)\<close> for \<theta>
-      by metis
-    show \<open>norm (F a) = norm a\<close>
-      using \<open>unitary U\<close> by (simp add: FU sandwich_def norm_isometry_o norm_isometry_o' tensor_op_norm)
-  qed
-  (* note this[cancel_with_type] *)
-  then show ?thesis
-    sorry
-qed
-
 lemma commutant_exchange:
-  fixes F :: \<open>'a update \<Rightarrow> 'b update\<close>
+  fixes F :: \<open>'a::finite update \<Rightarrow> 'b::finite update\<close>
   assumes \<open>iso_register F\<close>
   shows \<open>commutant (F ` X) = F ` commutant X\<close>
 proof (rule Set.set_eqI)
@@ -1215,25 +531,35 @@ proof (rule Set.set_eqI, rule iffI)
   then have comm: \<open>(a \<otimes>\<^sub>o id_cblinfun) *\<^sub>V x *\<^sub>V \<psi> = x *\<^sub>V (a \<otimes>\<^sub>o id_cblinfun) *\<^sub>V \<psi>\<close> for a \<psi>
     by (metis (mono_tags, lifting) commutant_def mem_Collect_eq rangeI cblinfun_apply_cblinfun_compose)
 
-  define op where \<open>op = classical_operator (\<lambda>i. Some (\<gamma>,i::'b))\<close>
-  have [simp]: \<open>classical_operator_exists (\<lambda>i. Some (\<gamma>,i))\<close>
-    apply (rule classical_operator_exists_inj)
-    using inj_map_def by blast
-  define x' where \<open>x' = op* o\<^sub>C\<^sub>L x o\<^sub>C\<^sub>L op\<close>
-  have x': \<open>cinner (ket j) (x' *\<^sub>V ket l) = cinner (ket (\<gamma>,j)) (x *\<^sub>V ket (\<gamma>,l))\<close> for j l
-    by (simp add: x'_def op_def classical_operator_ket cinner_adj_right)
+  obtain x' where x': \<open>cinner (ket j) (x' *\<^sub>V ket l) = cinner (ket (\<gamma>,j)) (x *\<^sub>V ket (\<gamma>,l))\<close> for j l
+  proof atomize_elim
+    obtain \<psi> where \<psi>: \<open>cinner (ket j) (\<psi> l) = cinner (ket (\<gamma>, j)) (x *\<^sub>V ket (\<gamma>, l))\<close> for l j
+      apply (atomize_elim, rule choice, rule allI)
+      apply (rule_tac x=\<open>Abs_ell2 (\<lambda>j. cinner (ket (\<gamma>, j)) (x *\<^sub>V ket (\<gamma>, l)))\<close> in exI)
+      by (simp add: cinner_ket_left Abs_ell2_inverse)
+    obtain x' where \<open>x' *\<^sub>V ket l = \<psi> l\<close> for l
+      apply atomize_elim
+      apply (rule exI[of _ \<open>cblinfun_extension (range ket) (\<lambda>l. \<psi> (inv ket l))\<close>])
+      apply (subst cblinfun_extension_apply)
+        apply (rule cblinfun_extension_exists_finite_dim)
+      by (auto simp add: inj_ket cindependent_ket)
+    with \<psi> have \<open>cinner (ket j) (x' *\<^sub>V ket l) = cinner (ket (\<gamma>, j)) (x *\<^sub>V ket (\<gamma>, l))\<close> for j l
+      by auto
+    then show \<open>\<exists>x'. \<forall>j l. cinner (ket j) (x' *\<^sub>V ket l) = cinner (ket (\<gamma>, j)) (x *\<^sub>V ket (\<gamma>, l))\<close>
+      by auto
+  qed
 
   have \<open>cinner (ket (i,j)) (x *\<^sub>V ket (k,l)) = cinner (ket (i,j)) ((id_cblinfun \<otimes>\<^sub>o x') *\<^sub>V ket (k,l))\<close> for i j k l
   proof -
     have \<open>cinner (ket (i,j)) (x *\<^sub>V ket (k,l))
         = cinner ((butterket i \<gamma> \<otimes>\<^sub>o id_cblinfun) *\<^sub>V ket (\<gamma>,j)) (x *\<^sub>V (butterket k \<gamma> \<otimes>\<^sub>o id_cblinfun) *\<^sub>V ket (\<gamma>,l))\<close>
-      by (auto simp: tensor_op_ket tensor_ell2_ket)
+      by (auto simp: tensor_op_ket)
     also have \<open>\<dots> = cinner (ket (\<gamma>,j)) ((butterket \<gamma> i \<otimes>\<^sub>o id_cblinfun) *\<^sub>V x *\<^sub>V (butterket k \<gamma> \<otimes>\<^sub>o id_cblinfun) *\<^sub>V ket (\<gamma>,l))\<close>
       by (metis (no_types, lifting) cinner_adj_left butterfly_adjoint id_cblinfun_adjoint tensor_op_adjoint)
     also have \<open>\<dots> = cinner (ket (\<gamma>,j)) (x *\<^sub>V (butterket \<gamma> i \<otimes>\<^sub>o id_cblinfun o\<^sub>C\<^sub>L butterket k \<gamma> \<otimes>\<^sub>o id_cblinfun) *\<^sub>V ket (\<gamma>,l))\<close>
       unfolding comm by (simp add: cblinfun_apply_cblinfun_compose)
     also have \<open>\<dots> = cinner (ket i) (ket k) * cinner (ket (\<gamma>,j)) (x *\<^sub>V ket (\<gamma>,l))\<close>
-      by (simp add: comp_tensor_op tensor_op_ket tensor_op_scaleC_left cinner_ket tensor_ell2_ket)
+      by (simp add: comp_tensor_op tensor_op_ket tensor_op_scaleC_left)
     also have \<open>\<dots> = cinner (ket i) (ket k) * cinner (ket j) (x' *\<^sub>V ket l)\<close>
       by (simp add: x')
     also have \<open>\<dots> = cinner (ket (i,j)) ((id_cblinfun \<otimes>\<^sub>o x') *\<^sub>V ket (k,l))\<close>
@@ -1270,98 +596,8 @@ proof -
     by (simp add: commutant_exchange commutant_tensor1)
 qed
 
-(* lemma TMP: \<open>isCont f a \<longleftrightarrow> filterlim f (nhds a) (nhds (f a))\<close>
-  apply rule
-  defer
-  by - *)
-
-(* definition Collect_in where \<open>Collect_in S P = {x\<in>S. P x}\<close> for S and P
-
-lemma Collect_in_parametric[transfer_rule]:
-  includes lifting_syntax
-  shows \<open>(rel_set R ===> (R ===> (\<longleftrightarrow>)) ===> rel_set R) Collect_in Collect_in\<close>
-  apply (auto intro!: simp: rel_fun_def rel_set_def Collect_in_def)
-  by blast+
-
-term Set.filter *)
-
-definition \<open>opensets = Collect open\<close>
-  \<comment> \<open>This behaves more nicely with the @{method transfer}-method (and friends) than \<^const>\<open>open\<close>.
-      So when rewriting a subgoal, using, e.g., \<^term>\<open>\<exists>U\<in>opensets. xxx\<close> instead of \<^term>\<open>\<exists>U. open U \<longrightarrow> xxx\<close> can make @{method transfer} work better. \<close>
-
-lemma opensets_parametric[transfer_rule]:
-  includes lifting_syntax
-  assumes [transfer_rule]: \<open>bi_unique R\<close>
-  assumes [transfer_rule]: \<open>(rel_set R ===> (\<longleftrightarrow>)) open open\<close>
-  shows \<open>(rel_set (rel_set R)) opensets opensets\<close>
-  using assms apply (simp add: opensets_def rel_set_def )
-  apply auto
-sorry
-
-
-(* TODO move *)
-(* TODO reprove concrete nhds transfer rules with this (or drop them?) *)
-lemma nhds_parametric[transfer_rule]:
-  includes lifting_syntax
-  assumes [transfer_rule]: \<open>bi_unique R\<close>
-  assumes [transfer_rule]: \<open>(rel_set R ===> (\<longleftrightarrow>)) open open\<close>
-  shows \<open>(R ===> rel_filter R) nhds nhds\<close>
-(* proof -
-  have \<open>(R ===> rel_filter R) (\<lambda>a. \<Sqinter> (principal ` Set.filter ((\<in>) a) opensets)) (\<lambda>a. \<Sqinter> (principal ` Set.filter ((\<in>) a) opensets))\<close>
-  show ?thesis
-    unfolding nhds_def
-    apply transfer_prover_start
-
-
-         apply transfer_step
-  apply transfer_step
-      apply transfer_step
-  apply transfer_step
-  apply transfer_step
-     apply (rule RelI)
-
-     apply transfer_step
-
-
-
-  term nhds *)
-  sorry
-
-lemma at_within_parametric[transfer_rule]: 
-  includes lifting_syntax
-  assumes [transfer_rule]: \<open>bi_unique R\<close>
-  assumes [transfer_rule]: \<open>(rel_set R ===> (\<longleftrightarrow>)) open open\<close>
-  shows \<open>(R ===> rel_set R ===> rel_filter R) at_within at_within\<close>
-  unfolding at_within_def
-  apply transfer_prover_start
-  apply transfer_step
-  apply transfer_step
-      apply transfer_step
-  apply transfer_step
-  apply transfer_step
-
-
-    apply transfer_step
-  apply transfer_step
-
-  
-  sorry
-
-
-  term at_within
-
-
-
-lemma transfer_nhds_weak_star_topology[transfer_rule]:
-  includes lifting_syntax
-  shows \<open>(cr_cblinfun_weak_star ===> rel_set cr_cblinfun_weak_star ===> rel_filter cr_cblinfun_weak_star) (at_within_in weak_star_topology) nhds\<close>
-  unfolding nhds_def nhdsin_def
-  apply (simp add: weak_star_topology_topspace)
-  by transfer_prover
-
-
 lemma same_range_equivalent:
-  fixes F :: \<open>'a update \<Rightarrow> 'c update\<close> and G :: \<open>'b update \<Rightarrow> 'c update\<close>
+  fixes F :: \<open>'a::finite update \<Rightarrow> 'c::finite update\<close> and G :: \<open>'b::finite update \<Rightarrow> 'c::finite update\<close>
   assumes [simp]: \<open>register F\<close> and [simp]: \<open>register G\<close>
   assumes \<open>range F = range G\<close>
   shows \<open>equivalent_registers F G\<close>
@@ -1372,10 +608,8 @@ proof -
     by (simp add: assms(3)[symmetric])
   have [simp]: \<open>inj F\<close> and [simp]: \<open>inj G\<close>
     by (simp_all add: register_inj)
-  have [simp]: \<open>bounded_clinear F\<close> \<open>bounded_clinear G\<close>
-    by (simp_all add: register_bounded_clinear)
   have [simp]: \<open>clinear F\<close> \<open>clinear G\<close>
-    by (simp_all add: bounded_clinear.clinear)
+    by simp_all
   define I J where \<open>I x = inv F (G x)\<close> and \<open>J y = inv G (F y)\<close> for x y
   have addI: \<open>I (x + y) = I x + I y\<close> for x y
     unfolding I_def
@@ -1437,41 +671,13 @@ proof -
     apply (subst register_adjoint[OF \<open>register G\<close>])
     apply (subst Hilbert_Choice.f_inv_into_f[where f=G], simp)+
     using assms(1) register_adjoint by blast
-  have normI: \<open>norm (I a) = norm a\<close> for a
-    unfolding I_def
-    by (metis G_rangeF assms(1) assms(2) f_inv_into_f register_norm)
-  have normJ: \<open>norm (J a) = norm a\<close> for a
-    unfolding J_def
-    by (metis F_rangeG assms(1) assms(2) f_inv_into_f register_norm)
-  have weak_star_I: \<open>continuous_map weak_star_topology weak_star_topology I\<close>
-  proof -
-    include lifting_syntax
-    define I' where \<open>I' = to_weak_star o I o from_weak_star\<close>
-    have [transfer_rule]: \<open>(cr_cblinfun_weak_star ===> cr_cblinfun_weak_star) I I'\<close>
-      by (metis (no_types, lifting) I'_def UNIV_I cr_cblinfun_weak_star_def o_def rel_funI to_weak_star_inverse)
-    have \<open>I' \<midarrow>a\<rightarrow> I' a\<close> for a
-      apply (transfer)
-      sorry
 
-      sorry
-    then have \<open>isCont I' a\<close> for a
-      by (simp add: continuous_within)
-    then have \<open>continuous_on UNIV I'\<close>
-      using continuous_at_imp_continuous_on by blast
-    then have \<open>continuous_map euclidean euclidean I'\<close>
-      using continuous_map_iff_continuous2 by blast
-    then show ?thesis
-      by transfer
-  qed
-  have weak_star_J: \<open>continuous_map weak_star_topology weak_star_topology J\<close>
-    sorry
-
-  from addI scaleI unitalI multI adjI normI weak_star_I
+  from addI scaleI unitalI multI adjI
   have \<open>register I\<close>
-    unfolding register_def by (auto intro!: bounded_clinearI[where K=1])
-  from addJ scaleJ unitalJ multJ adjJ normJ weak_star_J
+    unfolding register_def by (auto intro!: clinearI)
+  from addJ scaleJ unitalJ multJ adjJ
   have \<open>register J\<close>
-    unfolding register_def by (auto intro!: bounded_clinearI[where K=1])
+    unfolding register_def by (auto intro!: clinearI)
 
   have \<open>I o J = id\<close>
     unfolding I_def J_def o_def
